Proved soundness of bv2z_spec.

src/SSA2ZSSA.v
@@ -8,67 +8,174 @@ From nbits Require Import NBits.
 
 (** Conversion from a specification to a range specification, an algebraic specification, and a safety condition. *)
 
+Set Implicit Arguments.
+Unset Strict Implicit.
+Import Prenex Implicits.
+
+Record options : Set :=
+  mkOptions { add_carry_constraints : bool }.
+
+Definition default_options : options :=
+  {| add_carry_constraints := false |}.
 
 
-(* Safety conditions *)
+
+(* Tactics *)
+
+Ltac case_pairs :=
+  match goal with
+  | H : (_, _) = (_, _) |- _ => case: H; move=> ? ?; subst
+  | H : (if ?e then _ else _) = _ |- _ => move: H; case: e; intros
+  | H : (match ?t with | Tuint _ => _ | Tsint _ => _ end) = _ |- _ =>
+    move: H; case: t; intros
+  | H : (let (_, _) := Z.div_eucl ?e1 ?e2 in _) = (_, _) |- _ =>
+    let q := fresh "q" in
+    let r := fresh "r" in
+    let Hqr := fresh in
+    move: H; dcase (Z.div_eucl e1 e2) => [[q r] Hqr]; intros
+  end.
+
+Ltac case_svar_notin :=
+  match goal with
+  | H : svar_notin ?v (SSAVS.singleton _) |- _ =>
+    move/svar_notin_singleton: H => H
+  | H : svar_notin ?v (SSAVS.add _ _) |- _ =>
+    let H1 := fresh in let H2 := fresh in
+    move/svar_notin_add: H => [H1 H2]
+  | H : svar_notin ?v (SSAVS.union _ _) |- _ =>
+    let H1 := fresh in let H2 := fresh in
+    move/svar_notin_union: H => [H1 H2]
+  end.
+
+
+(** Generate new SSA variable names *)
+
+Section GenSvar.
+
+  Import SSA.
+
+  Definition max_svar (vs : SSAVS.t) : VarOrder.t :=
+    match SSAVS.max_elt vs with
+    | Some v => svar v
+    | None => 0%num
+    end.
+
+  Definition new_svar (vs : SSAVS.t) : VarOrder.t :=
+    N.succ (max_svar vs).
+
+  Definition new_svar_program (p : program) : VarOrder.t :=
+    N.succ (max_svar (vars_program p)).
+
+  Lemma N_ltb_succ v : (v <? N.succ v)%num.
+  Proof. apply: (proj2 (N.ltb_lt v (N.succ v))). exact: N.lt_succ_diag_r. Qed.
+
+  Lemma V_ltb_succ v i j : SSAVarOrder.ltn (v, j) ((N.succ v), i).
+  Proof.
+    rewrite /SSAVarOrder.ltn /SSAVarOrder.M.ltn /VarOrder.ltn /NOrderMinimal.ltn /=.
+    rewrite N_ltb_succ. exact: is_true_true.
+  Qed.
+
+  Lemma new_svar_notin vs : svar_notin (new_svar vs) vs.
+  Proof.
+    rewrite /new_svar /max_svar. set x := SSAVS.max_elt vs.
+    have: SSAVS.max_elt vs = x by reflexivity. case x.
+    - move=> v Hmax i. apply/negP => Hmem. apply: (VSLemmas.max_elt2 Hmax Hmem).
+      exact: V_ltb_succ.
+    - move=> Hnone i. apply: VSLemmas.is_empty_mem.
+      exact: (VSLemmas.max_elt3 Hnone).
+  Qed.
+
+  Lemma new_svar_notin_program p :
+    svar_notin (new_svar_program p) (vars_program p).
+  Proof. exact: new_svar_notin. Qed.
+
+End GenSvar.
+
+
+
+(** Safety conditions *)
 
 Section Safety.
 
   Import SSA.
 
-  Definition uaddB_safe bs1 bs2 : bool := ~~ carry_addB bs1 bs2 .
+  Definition uaddB_safe bs1 bs2 : bool := ~~ carry_addB bs1 bs2.
 
-  Definition saddB_safe bs1 bs2 : bool := ~~ Saddo bs1 bs2 .
+  Definition saddB_safe bs1 bs2 : bool := ~~ Saddo bs1 bs2.
 
   Definition addB_safe typ_a bs1 bs2 : bool :=
     if Typ.is_unsigned typ_a then uaddB_safe bs1 bs2
-    else saddB_safe bs1 bs2 .
+    else saddB_safe bs1 bs2.
+
+  Definition adds_safe typ_a bs1 bs2 : bool :=
+    if Typ.is_unsigned typ_a then true
+    else saddB_safe bs1 bs2.
 
   Definition uadcB_safe bs1 bs2 c : bool :=
-    ~~ carry_addB bs1 bs2 && ~~ carry_addB (addB bs1 bs2) c .
+    ~~ carry_addB bs1 bs2 && ~~ carry_addB (addB bs1 bs2) c.
 
   Definition sadcB_safe bs1 bs2 c : bool :=
-    ~~ Saddo bs1 bs2 && ~~ Saddo (addB bs1 bs2) c .
+    ~~ Saddo bs1 bs2 && ~~ Saddo (addB bs1 bs2) c.
 
   Definition adcB_safe typ_a bs1 bs2 bsc : bool :=
     if Typ.is_unsigned typ_a then uadcB_safe bs1 bs2 bsc
-    else sadcB_safe bs1 bs2 bsc .
+    else sadcB_safe bs1 bs2 bsc.
 
-  Definition usubB_safe bs1 bs2 : bool := ~~ borrow_subB bs1 bs2 .
+  Definition adcs_safe typ_a bs1 bs2 bsc : bool :=
+    if Typ.is_unsigned typ_a then true
+    else sadcB_safe bs1 bs2 bsc.
 
-  Definition ssubB_safe bs1 bs2 : bool := ~~ Ssubo bs1 bs2 .
+  Definition usubB_safe bs1 bs2 : bool := ~~ borrow_subB bs1 bs2.
+
+  Definition ssubB_safe bs1 bs2 : bool := ~~ Ssubo bs1 bs2.
 
   Definition subB_safe typ_a bs1 bs2 : bool :=
     if Typ.is_unsigned typ_a then usubB_safe bs1 bs2
-    else ssubB_safe bs1 bs2 .
+    else ssubB_safe bs1 bs2.
+
+  Definition subc_safe typ_a bs1 bs2 : bool :=
+    if Typ.is_unsigned typ_a then true
+    else ssubB_safe bs1 bs2.
+
+  Definition subb_safe typ_a bs1 bs2 : bool :=
+    if Typ.is_unsigned typ_a then true
+    else ssubB_safe bs1 bs2.
 
   Definition usbbB_safe bs1 bs2 c : bool :=
-    ~~ borrow_subB bs1 bs2 && ~~ borrow_subB (subB bs1 bs2) c .
+    ~~ borrow_subB bs1 bs2 && ~~ borrow_subB (subB bs1 bs2) c.
 
   Definition ssbbB_safe bs1 bs2 c : bool :=
-    ~~ Ssubo bs1 bs2 && ~~ Ssubo (subB bs1 bs2) c .
+    ~~ Ssubo bs1 bs2 && ~~ Ssubo (subB bs1 bs2) c.
 
   Definition sbbB_safe typ_a bs1 bs2 bsb : bool :=
     if Typ.is_unsigned typ_a then usbbB_safe bs1 bs2 bsb
-    else ssbbB_safe bs1 bs2 bsb .
+    else ssbbB_safe bs1 bs2 bsb.
+
+  Definition sbbs_safe typ_a bs1 bs2 bsb : bool :=
+    if Typ.is_unsigned typ_a then true
+    else ssbbB_safe bs1 bs2 bsb.
 
   Definition usbcB_safe bs1 bs2 c : bool :=
-    ~~ borrow_subB bs1 bs2 && ~~ borrow_subB (subB bs1 bs2) (subB (ones 1) c) .
+    ~~ borrow_subB bs1 bs2 && ~~ borrow_subB (subB bs1 bs2) (subB (ones 1) c).
 
   Definition ssbcB_safe bs1 bs2 c : bool :=
-    ~~ Ssubo bs1 bs2 && ~~ Ssubo (subB bs1 bs2) (subB (ones 1) c) .
+    ~~ Ssubo bs1 bs2 && ~~ Ssubo (subB bs1 bs2) (subB (ones 1) c).
 
   Definition sbcB_safe typ_a bs1 bs2 bsc : bool :=
     if Typ.is_unsigned typ_a then usbcB_safe bs1 bs2 bsc
-    else ssbcB_safe bs1 bs2 bsc .
+    else ssbcB_safe bs1 bs2 bsc.
 
-  Definition umulB_safe bs1 bs2 : bool := ~~ Umulo bs1 bs2 .
+  Definition sbcs_safe typ_a bs1 bs2 bsc : bool :=
+    if Typ.is_unsigned typ_a then true
+    else ssbcB_safe bs1 bs2 bsc.
 
-  Definition smulB_safe bs1 bs2 : bool := ~~ Smulo bs1 bs2 .
+  Definition umulB_safe bs1 bs2 : bool := ~~ Umulo bs1 bs2.
+
+  Definition smulB_safe bs1 bs2 : bool := ~~ Smulo bs1 bs2.
 
   Definition mulB_safe typ_a bs1 bs2 : bool :=
     if Typ.is_unsigned typ_a then umulB_safe bs1 bs2
-    else smulB_safe bs1 bs2 .
+    else smulB_safe bs1 bs2.
 
   Definition ushlBn_safe bs n : bool := high n bs == zeros n.
 
@@ -115,14 +222,26 @@ Section Safety.
     match i with
     | Iadd _ a1 a2 =>
       addB_safe (atyp a1 te) (eval_atomic a1 s) (eval_atomic a2 s)
+    | Iadds _ _ a1 a2 =>
+      adds_safe (atyp a1 te) (eval_atomic a1 s) (eval_atomic a2 s)
     | Iadc _ a1 a2 ac =>
       adcB_safe (atyp a1 te) (eval_atomic a1 s) (eval_atomic a2 s) (eval_atomic ac s)
+    | Iadcs _ _ a1 a2 ac =>
+      adcs_safe (atyp a1 te) (eval_atomic a1 s) (eval_atomic a2 s) (eval_atomic ac s)
     | Isub _ a1 a2 =>
       subB_safe (atyp a1 te) (eval_atomic a1 s) (eval_atomic a2 s)
+    | Isubc _ _ a1 a2 =>
+      subc_safe (atyp a1 te) (eval_atomic a1 s) (eval_atomic a2 s)
+    | Isubb _ _ a1 a2 =>
+      subb_safe (atyp a1 te) (eval_atomic a1 s) (eval_atomic a2 s)
     | Isbc _ a1 a2 ac =>
       sbcB_safe (atyp a1 te) (eval_atomic a1 s) (eval_atomic a2 s) (eval_atomic ac s)
     | Isbb _ a1 a2 ab =>
       sbbB_safe (atyp a1 te) (eval_atomic a1 s) (eval_atomic a2 s) (eval_atomic ab s)
+    | Isbcs _ _ a1 a2 ac =>
+      sbcs_safe (atyp a1 te) (eval_atomic a1 s) (eval_atomic a2 s) (eval_atomic ac s)
+    | Isbbs _ _ a1 a2 ab =>
+      sbbs_safe (atyp a1 te) (eval_atomic a1 s) (eval_atomic a2 s) (eval_atomic ab s)
     | Imul _ a1 a2 =>
       mulB_safe (atyp a1 te) (eval_atomic a1 s) (eval_atomic a2 s)
     | Ishl _ a n =>
@@ -135,12 +254,6 @@ Section Safety.
     | Inondet _ _
     | Imov _ _
     | Icmov _ _ _ _
-    | Iadds _ _ _ _
-    | Iadcs _ _ _ _ _
-    | Isubc _ _ _ _
-    | Isubb _ _ _ _
-    | Isbcs _ _ _ _ _
-    | Isbbs _ _ _ _ _
     | Imull _ _ _ _
     | Imulj _ _ _
     | Inot _ _ _
@@ -151,7 +264,7 @@ Section Safety.
     | Ijoin _ _ _
     | Icast _ _ _
     | Iassume _ => true
-    end .
+    end.
 
   Inductive ssa_program_safe_at : SSATE.env -> program -> SSAStore.t -> Prop :=
   | ssa_program_safe_at_nil te s :
@@ -160,43 +273,103 @@ Section Safety.
       ssa_instr_safe_at te hd s ->
       (forall s', eval_instr te hd s s' ->
                   ssa_program_safe_at (instr_succ_typenv hd te) tl s') ->
-      ssa_program_safe_at te (hd::tl) s .
+      ssa_program_safe_at te (hd::tl) s.
 
   Definition ssa_program_safe te p : Prop :=
-    forall s, ssa_program_safe_at te p s .
+    forall s, ssa_program_safe_at te p s.
 
   Definition ssa_spec_safe sp :=
     forall s, eval_rbexp (rng_bexp (spre sp)) s ->
-              ssa_program_safe_at (sinputs sp) (sprog sp) s .
+              ssa_program_safe_at (sinputs sp) (sprog sp) s.
+
+
+  Lemma ssa_instr_safe_at_eqn E i s :
+    ssa_instr_safe_at E i s -> ssa_instr_safe_at E (eqn_instr i) s.
+  Proof. case: i => //=. move=> [] e r _ /=. by trivial. Qed.
 
 End Safety.
 
 
 
-(* Convert a bit-vector program to an integer program *)
+(** Conversion from SSA programs to algebraic expressions *)
 
-Section SSA2ZSSA.
+Section SSA2Algebra.
 
   Import SSA ZSSA.
+
+  Variable options : options.
+
+
+  Ltac split_disjoint :=
+    match goal with
+    | H : is_true (VSLemmas.disjoint _ (SSAVS.singleton _)) |- _ =>
+      rewrite VSLemmas.disjoint_singleton in H
+    | H : is_true (VSLemmas.disjoint _ (SSAVS.add _ _)) |- _ =>
+      let H1 := fresh "Hdisj" in let H2 := fresh "Hdisj" in
+      rewrite VSLemmas.disjoint_add in H;
+      move/andP: H => [H1 H2]
+    end.
+
 
   Definition bv2z_atomic (a : atomic) : zexp :=
     match a with
     | Avar v => evar v
-    | Aconst ty bs =>
-      match ty with
-      | Tuint _ => econst (to_Zpos bs)
-      | Tsint _ => econst (to_Z bs)
-      end
+    | Aconst ty bs => econst (bv2z ty bs)
     end.
 
-  Definition bv2z_assign v e := eeq (evar v) e.
-  Definition bv2z_join e h l p := eeq (eadd l (emul2p h p)) e.
-  Definition bv2z_split vh vl e p := bv2z_join e (evar vh) (evar vl) p.
-  Definition bv2z_is_carry c := eeq (emul (evar c) (esub (evar c) (econst 1)))
-                                    (econst 0).
-  Definition carry_constr b c := if b then [:: bv2z_is_carry c] else [::].
+  Definition bv2z_assign (v : ssavar) (e : SSA.eexp) := eeq (evar v) e.
+  Definition bv2z_join (e h l : SSA.eexp) (p : nat) :=
+    eeq (eadd l (emul2p h (Z.of_nat p))) e.
+  Definition bv2z_split (vh vl : ssavar) (e : SSA.eexp) (p : nat) :=
+    bv2z_join e (evar vh) (evar vl) p.
+  Definition bv2z_is_carry (c : ssavar) :=
+    eeq (emul (evar c) (esub (evar c) (econst 1)))
+        (econst 0).
+  Definition carry_constr (c : ssavar) :=
+    if (add_carry_constraints options) then [:: bv2z_is_carry c] else [::].
 
-  Definition bv2z_instr (te : SSATE.env) (nvar : N) (g : N) (i : instr) :
+  Definition bv2z_cast (avn : VarOrder.t) (g : N) v vtyp a atyp :=
+    match vtyp, atyp with
+    | Tuint wv, Tuint wa =>
+      if wv >= wa then
+        (g, [:: Eeq (evar v) (bv2z_atomic a)])
+      else
+        let discarded := (avn, g) in
+        let g' := N.succ g in
+        (g', [:: bv2z_split discarded v (bv2z_atomic a) wv])
+    | Tuint wv, Tsint wa =>
+      (* a_sign and discarded have different meanings but
+         the polynomial equation is equivalent. *)
+      if wv >= wa then
+        let a_sign := (avn, g) in
+        let g' := N.succ g in
+        (g', [:: bv2z_join (evar v) (evar a_sign) (bv2z_atomic a) wv])
+      else
+        let discarded := (avn, g) in
+        let g' := N.succ g in
+        (g', [:: bv2z_split discarded v (bv2z_atomic a) wv])
+    | Tsint wv, Tuint wa =>
+      if wv > wa then
+        (g, [:: Eeq (evar v) (bv2z_atomic a)])
+      else
+        let discarded := (avn, g) in
+        let g' := N.succ g in
+        (g', [:: bv2z_split discarded v (bv2z_atomic a) wv])
+    | Tsint wv, Tsint wa =>
+      if wv >= wa then
+        (g, [:: Eeq (evar v) (bv2z_atomic a)])
+      else
+        let discarded := (avn, g) in
+        let g' := N.succ g in
+        (g', [:: bv2z_split discarded v (bv2z_atomic a) wv])
+    end.
+
+  Definition bv2z_vpc (avn : VarOrder.t) (g : N) (v : ssavar) a :=
+    (g, [:: Eeq (evar v) (bv2z_atomic a)]).
+
+  (* avn: the name of auxiliary variables
+     g: the SSA index of the next auxiliary variable *)
+  Definition bv2z_instr (te : SSATE.env) (avn : VarOrder.t) (g : N) (i : instr) :
     (N * seq ebexp) :=
     match i with
     | Imov v a =>
@@ -210,12 +383,31 @@ Section SSA2ZSSA.
       let za2 := bv2z_atomic a2 in
       let a2size := asize a2 te in
       (g, [:: bv2z_split vh vl (eadd (emul2p za1 (Z.of_nat a2size)) za2)
-              (Z.of_nat (a2size - n))])
-    | Inondet v t => (g, [::])
+              (a2size - n)])
+    | Inondet v t =>
+      if t == Tbit then (g, carry_constr v)
+      else (g, [::])
     | Icmov v c a1 a2 =>
-      (g, [::])
+      let zc := bv2z_atomic c in
+      let za1 := bv2z_atomic a1 in
+      let za2 := bv2z_atomic a2 in
+      (g, [:: bv2z_assign
+              v
+              (eadd (emul zc za1)
+                    (emul (esub (econst Z.one) zc) za2))])
     | Inop => (g, [::])
-    | Inot v t a => (g, [::])
+    | Inot v t a =>
+      let za := bv2z_atomic a in
+      match t with
+      | Tuint w =>
+        (g, [:: bv2z_assign
+                v
+                (esub (econst (Z.sub (z2expn (Z.of_nat w)) Z.one)) za)])
+      | Tsint w =>
+        (g, [:: bv2z_assign
+                v
+                (esub (eneg za) (econst Z.one))])
+      end
     | Iadd v a1 a2 =>
       let za1 := bv2z_atomic a1 in
       let za2 := bv2z_atomic a2 in
@@ -223,8 +415,13 @@ Section SSA2ZSSA.
     | Iadds c v a1 a2 =>
       let za1 := bv2z_atomic a1 in
       let za2 := bv2z_atomic a2 in
-      let a2size := asize a2 te in
-      (g, [:: bv2z_split c v (eadd za1 za2) (Z.of_nat a2size)])
+      match atyp a1 te with
+      | Tuint w =>
+        (g, [:: bv2z_split c v (eadd za1 za2) w]
+              ++ (carry_constr c))
+      | Tsint w =>
+        (g, [:: bv2z_assign v (eadd za1 za2)])
+      end
     | Iadc v a1 a2 y =>
       let za1 := bv2z_atomic a1 in
       let za2 := bv2z_atomic a2 in
@@ -234,33 +431,2233 @@ Section SSA2ZSSA.
       let za1 := bv2z_atomic a1 in
       let za2 := bv2z_atomic a2 in
       let zy := bv2z_atomic y in
-      let a2size := asize a2 te in
-      (g, [::])
+      match atyp a1 te with
+      | Tuint w =>
+        (g, [:: bv2z_split c v (eadd (eadd za1 za2) zy) w]
+              ++ (carry_constr c))
+      | Tsint w =>
+        (g, [:: bv2z_assign v (eadd (eadd za1 za2) zy)])
+      end
     | Isub v a1 a2 =>
       let za1 := bv2z_atomic a1 in
       let za2 := bv2z_atomic a2 in
       (g, [:: bv2z_assign v (esub za1 za2)])
-    | Isubc c v a1 a2 => (g, [::])
-    | Isubb c v a1 a2 => (g, [::])
-    | Isbc v a1 a2 y => (g, [::])
-    | Isbcs c v a1 a2 y => (g, [::])
-    | Isbb v a1 a2 y => (g, [::])
-    | Isbbs c v a1 a2 y => (g, [::])
-    | Imul v a1 a2 => (g, [::])
-    | Imull vh vl a1 a2 => (g, [::])
-    | Imulj v a1 a2 => (g, [::])
-    | Isplit vh vl a n => (g, [::])
-    | Iand v t a1 a2 => (g, [::])
-    | Ior v t a1 a2 => (g, [::])
-    | Ixor v t a1 a2 => (g, [::])
-    | Icast v t a => (g, [::])
-    | Ivpc v t a => (g, [::])
-    | Ijoin v ah al => (g, [::])
-    | Iassume e => (g, [::])
+    | Isubc c v a1 a2 =>
+      let za1 := bv2z_atomic a1 in
+      let za2 := bv2z_atomic a2 in
+      match atyp a1 te with
+      | Tuint w =>
+        (g, [:: bv2z_join
+                (evar v) (esub (econst Z.one) (evar c))
+                (esub za1 za2) w]
+              ++ (carry_constr c))
+      | Tsint w =>
+        (g, [:: bv2z_assign v (esub za1 za2)])
+      end
+    | Isubb c v a1 a2 =>
+      let za1 := bv2z_atomic a1 in
+      let za2 := bv2z_atomic a2 in
+      match atyp a1 te with
+      | Tuint w =>
+        (g, [:: bv2z_join (evar v) (evar c) (esub za1 za2) w]
+              ++ (carry_constr c))
+      | Tsint w =>
+        (g, [:: bv2z_assign v (esub za1 za2)])
+      end
+    | Isbc v a1 a2 y =>
+      let za1 := bv2z_atomic a1 in
+      let za2 := bv2z_atomic a2 in
+      let zy := bv2z_atomic y in
+      (g, [:: bv2z_assign v (esub (esub za1 za2) (esub (econst Z.one) zy))])
+    | Isbcs c v a1 a2 y =>
+      let za1 := bv2z_atomic a1 in
+      let za2 := bv2z_atomic a2 in
+      let zy := bv2z_atomic y in
+      match atyp a1 te with
+      | Tuint w =>
+        (g, [:: bv2z_join
+                (evar v) (esub (econst Z.one) (evar c))
+                (esub (esub za1 za2) (esub (econst Z.one) zy)) w]
+              ++ (carry_constr c))
+      | Tsint w =>
+        (g, [:: bv2z_assign v (esub (esub za1 za2) (esub (econst Z.one) zy))])
+      end
+    | Isbb v a1 a2 y =>
+      let za1 := bv2z_atomic a1 in
+      let za2 := bv2z_atomic a2 in
+      let zy := bv2z_atomic y in
+      (g, [:: bv2z_assign v (esub (esub za1 za2) (esub (econst Z.one) zy))])
+    | Isbbs c v a1 a2 y =>
+      let za1 := bv2z_atomic a1 in
+      let za2 := bv2z_atomic a2 in
+      let zy := bv2z_atomic y in
+      match atyp a1 te with
+      | Tuint w =>
+        (g, [:: bv2z_join
+                (esub (esub za1 za2) zy) (eneg (evar c))
+                (evar v) w]
+              ++ (carry_constr c))
+      | Tsint w =>
+        (g, [:: bv2z_assign v (esub (esub za1 za2) zy)])
+      end
+    | Imul v a1 a2 =>
+      let za1 := bv2z_atomic a1 in
+      let za2 := bv2z_atomic a2 in
+      (g, [:: bv2z_assign v (emul za1 za2)])
+    | Imull vh vl a1 a2 =>
+      let za1 := bv2z_atomic a1 in
+      let za2 := bv2z_atomic a2 in
+      let a2size := asize a2 te in
+      (g, [:: bv2z_split vh vl (emul za1 za2) a2size])
+    | Imulj v a1 a2 =>
+      let za1 := bv2z_atomic a1 in
+      let za2 := bv2z_atomic a2 in
+      (g, [:: bv2z_assign v (emul za1 za2)])
+    | Isplit vh vl a n =>
+      let za := bv2z_atomic a in
+      (g, [:: bv2z_split vh vl za n])
+    | Iand v t a1 a2 => (g, [::]) (* cannot be translated to polynomials *)
+    | Ior v t a1 a2 => (g, [::]) (* cannot be translated to polynomials *)
+    | Ixor v t a1 a2 => (g, [::]) (* cannot be translated to polynomials *)
+    | Icast v t a => bv2z_cast avn g v t a (atyp a te)
+    | Ivpc v t a => bv2z_vpc avn g v a
+    | Ijoin v ah al =>
+      let zah := bv2z_atomic ah in
+      let zal := bv2z_atomic al in
+      let alsize := asize al te in
+      (g, [:: bv2z_join (evar v) zah zal alsize])
+    | Iassume e => (g, split_eand (eqn_bexp e))
     end.
 
-  (* TODO: see bv2z_program in certified_qhasm_vcg/mqhasm/bvSSA2zSSA.v *)
-  Definition bv2z_program (nvar : N) (idx : N) (p : program) : N * ZSSA.zprogram :=
-    (nvar, [::]).
+  Fixpoint bv2z_program (te : SSATE.env) (avn : VarOrder.t) (g : N) (p : program) :
+    N * seq ebexp :=
+    match p with
+    | [::] => (g, [::])
+    | hd::tl =>
+      let (g_hd, zhd) := bv2z_instr te avn g hd in
+      let (g_tl, ztl) := bv2z_program (instr_succ_typenv hd te) avn g_hd tl in
+      (g_tl, zhd ++ ztl)
+    end.
 
-End SSA2ZSSA.
+  Definition new_svar_espec (s : espec) : VarOrder.t :=
+    new_svar (SSAVS.union (vars_env (esinputs s))
+                          (SSAVS.union
+                             (vars_ebexp (espre s))
+                             (SSAVS.union (vars_program (esprog s))
+                                          (vars_ebexp (espost s))))).
+
+  Definition new_svar_spec (s : spec) : VarOrder.t :=
+    new_svar (SSAVS.union (vars_env (sinputs s))
+                          (SSAVS.union
+                             (vars_bexp (spre s))
+                             (SSAVS.union (vars_program (sprog s))
+                                          (vars_bexp (spost s))))).
+
+  Fixpoint aux_vars_lt_nat (avn : VarOrder.t) (gn : nat) : SSAVS.t :=
+    match gn with
+    | O => SSAVS.empty
+    | S n => SSAVS.add (avn, N.of_nat n) (aux_vars_lt_nat avn n)
+    end.
+
+  Definition aux_vars_lt (avn : VarOrder.t) (g : N) : SSAVS.t :=
+    aux_vars_lt_nat avn (N.to_nat g).
+
+  Definition bv2z_espec avn (s : espec) : zspec :=
+    let (g, eprogs) := bv2z_program (esinputs s)
+                                    avn initial_index (esprog s) in
+    {| zsinputs := SSAVS.union
+                     (aux_vars_lt avn g)
+                     (vars_env (program_succ_typenv (esprog s) (esinputs s)));
+       zspre := eand (espre s) (eands eprogs);
+       zsprog := [::];
+       zspost := espost s |}.
+
+
+  Lemma aux_vars_lt_nat_mem avn g n :
+    (N.to_nat n < g)%N -> SSAVS.mem (avn, n) (aux_vars_lt_nat avn g).
+  Proof.
+    elim: g n => //=. move=> g IH n H. case Hn: (N.to_nat n == g).
+    - rewrite -(eqP Hn) Nnat.N2Nat.id. exact: (SSAVS.Lemmas.mem_add_eq (eqxx _)).
+    - rewrite ltnS leq_eqVlt Hn /= in H. apply: SSAVS.Lemmas.mem_add3.
+      exact: (IH _ H).
+  Qed.
+
+  Lemma aux_vars_lt_mem avn g n :
+    (n < g)%num -> SSAVS.mem (avn, n) (aux_vars_lt avn g).
+  Proof.
+    move=> H. apply: aux_vars_lt_nat_mem. apply/N2Nat_inj_lt. assumption.
+  Qed.
+
+  Lemma aux_vars_lt_nat_svar x avn g :
+    SSAVS.mem x (aux_vars_lt_nat avn g) -> svar x = avn.
+  Proof.
+    elim: g => [| g IH] Hmem //=. rewrite /= in Hmem.
+    case/SSAVS.Lemmas.mem_add1 : Hmem => Hmem.
+    - rewrite (eqP Hmem); reflexivity.
+    - exact: (IH Hmem).
+  Qed.
+
+  Lemma aux_vars_lt_svar x avn g :
+    SSAVS.mem x (aux_vars_lt avn g) -> svar x = avn.
+  Proof. exact: aux_vars_lt_nat_svar. Qed.
+
+  Lemma aux_vars_lt_nat_sidx x avn g :
+    SSAVS.mem x (aux_vars_lt_nat avn g) -> (sidx x < N.of_nat g)%num.
+  Proof.
+    elim: g => [| g IH] Hmem //=. rewrite /= in Hmem.
+    case/SSAVS.Lemmas.mem_add1 : Hmem => Hmem.
+    - rewrite (eqP Hmem) /=. rewrite Pos.of_nat_succ -positive_nat_N.
+      rewrite Nat2Pos.id; last by done. apply/N2Nat_inj_lt.
+      rewrite !Nnat.Nat2N.id. done.
+    - rewrite Pos.of_nat_succ -positive_nat_N. rewrite Nat2Pos.id; last by done.
+      apply: (N.lt_trans _ (N.of_nat g) _ (IH Hmem)).
+      apply/N2Nat_inj_lt. rewrite !Nnat.Nat2N.id. exact: ltnSn.
+  Qed.
+
+  Lemma aux_vars_lt_sidx x avn g :
+    SSAVS.mem x (aux_vars_lt avn g) -> (sidx x < g)%num.
+  Proof.
+    move=> H. move: (aux_vars_lt_nat_sidx H) => {H} H.
+    rewrite Nnat.N2Nat.id in H. assumption.
+  Qed.
+
+  Lemma aux_vars_lt_nat_subset avn g1 g2 :
+    (g1 <= g2)%N -> SSAVS.subset (aux_vars_lt_nat avn g1) (aux_vars_lt_nat avn g2).
+  Proof.
+    move=> H. apply: SSAVS.subset_1. move=> [vn vi] /SSAVS.Lemmas.memP Hmem.
+    apply/SSAVS.Lemmas.memP. move: (aux_vars_lt_nat_svar Hmem) => /= ->.
+    apply: aux_vars_lt_nat_mem. move: (aux_vars_lt_nat_sidx Hmem) => /= Hlt.
+    move/N2Nat_inj_lt: Hlt. rewrite Nnat.Nat2N.id => Hlt.
+    exact: (Nats.ltn_leq_trans Hlt H).
+  Qed.
+
+  Lemma aux_vars_lt_subset avn g1 g2 :
+    (g1 <= g2)%num -> SSAVS.subset (aux_vars_lt avn g1) (aux_vars_lt avn g2).
+  Proof.
+    move=> H. rewrite /aux_vars_lt. apply: aux_vars_lt_nat_subset.
+    apply/N2Nat_inj_le. assumption.
+  Qed.
+
+  Lemma vars_bv2z_atomic a : vars_zexp (bv2z_atomic a) = vars_atomic a.
+  Proof. by case: a. Qed.
+
+  Lemma vars_carry_constr c :
+    SSAVS.Equal
+      (vars_zbexp (eands (carry_constr c)))
+      (if add_carry_constraints options then SSAVS.singleton c else SSAVS.empty).
+  Proof.
+    rewrite /carry_constr. case: (add_carry_constraints options) => //=.
+    rewrite !SSAVS.Lemmas.union_emptyr. rewrite SSAVS.Lemmas.union_same.
+    reflexivity.
+  Qed.
+
+
+  Lemma bv2z_program_cons te avn g1 g2 i p zip :
+    (g2, zip) = bv2z_program te avn g1 (i::p) ->
+    exists g3, exists zi, exists zp,
+          (g3, zi) = bv2z_instr te avn g1 i /\
+          (g2, zp) = bv2z_program (instr_succ_typenv i te) avn g3 p /\
+          zip = zi ++ zp.
+  Proof.
+    rewrite /=. dcase (bv2z_instr te avn g1 i) => [[g_hd zhd] Hhd].
+    dcase (bv2z_program (instr_succ_typenv i te) avn g_hd p) => [[g_tl ztl] Htl].
+    case=> ? ?; subst. exists g_hd; exists zhd; exists ztl. done.
+  Qed.
+
+  Lemma bv2z_eqn_instr te avn g i :
+    bv2z_instr te avn g (eqn_instr i) = bv2z_instr te avn g i.
+  Proof. case: i => //=. by case=> [e r]. Qed.
+
+  Lemma bv2z_eqn_program te avn g p :
+    bv2z_program te avn g (eqn_program p) = bv2z_program te avn g p.
+  Proof.
+    elim: p te avn g => [| i p IH] te avn g //=.
+    dcase (bv2z_instr te avn g (eqn_instr i)) => [[g_hd zhd] Hhd].
+    dcase (bv2z_program (instr_succ_typenv (eqn_instr i) te) avn g_hd (eqn_program p))
+          => [[g_tl ztl] Htl]. dcase (bv2z_instr te avn g i) => [[g_hd0 zhd0] Hhd0].
+    dcase (bv2z_program (instr_succ_typenv i te) avn g_hd0 p) => [[g_tl0 ztl0] Htl0].
+    rewrite bv2z_eqn_instr Hhd0 in Hhd. case: Hhd => ? ?; subst.
+    rewrite IH SSA.eqn_instr_succ_typenv Htl0 in Htl. case: Htl => ? ?; subst.
+    reflexivity.
+  Qed.
+
+  Lemma bv2z_cast_idx_inc avn g1 g2 v t a ta zi :
+    bv2z_cast avn g1 v t a ta = (g2, zi) ->
+    (g1 <= g2)%num.
+  Proof.
+    rewrite /bv2z_cast. case: t; case: ta.
+    - move=> wv wa; case: (wv <= wa); case=> ? ?; subst.
+      + exact: N.le_refl.
+      + exact: N.le_succ_diag_r.
+    - move=> wv wa; case: (wv <= wa); case=> ? ?; subst.
+      + exact: N.le_succ_diag_r.
+      + exact: N.le_succ_diag_r.
+    - move=> wv wa; case: (wv < wa); case=> ? ?; subst.
+      + exact: N.le_refl.
+      + exact: N.le_succ_diag_r.
+    - move=> wv wa; case: (wv <= wa); case=> ? ?; subst.
+      + exact: N.le_refl.
+      + exact: N.le_succ_diag_r.
+  Qed.
+
+  Lemma bv2z_instr_idx_inc te avn g1 g2 i zi :
+    bv2z_instr te avn g1 i = (g2, zi) -> (g1 <= g2)%num.
+  Proof.
+    ((case: i => /=); intros;
+     (let rec tac :=
+          match goal with
+          | H : (_, _) = (_, _) |- _ => case: H => -> _; tac
+          | H : (if ?b then _ else _) = (_, _) |- _ =>
+            move: H; case: b; intro; tac
+          | H : (match ?t with | Tuint _ => _ | Tsint _ => _ end) = _ |- _ =>
+            move: H; case: t; intros; tac
+          | H : bv2z_cast _ _ _ _ _ _ = _ |- _ =>
+            exact: (bv2z_cast_idx_inc H)
+          | H : bv2z_vpc _ _ _ _ = _ |- _ => rewrite /bv2z_vpc in H; tac
+          | |- (?x <= ?x)%num => exact: N.le_refl
+          | |- _ => idtac
+          end in
+      tac)).
+  Qed.
+
+  Lemma bv2z_program_idx_inc te avn g1 g2 p zp :
+    bv2z_program te avn g1 p = (g2, zp) -> (g1 <= g2)%num.
+  Proof.
+    elim: p te g1 g2 zp => [te g1 g2 zp | hd tl IH te g1 g2 zp] /=.
+    - case=> -> _. exact: N.le_refl.
+    - dcase (bv2z_instr te avn g1 hd) => [[g_hd zhd] Hhd].
+      dcase (bv2z_program (instr_succ_typenv hd te) avn g_hd tl) => [[g_tl ztl] Htl].
+      case=> <- _. move: (bv2z_instr_idx_inc Hhd) => Hg1hd.
+      move: (IH _ _ _ _ Htl) => Hghdtl. exact: (N.le_trans _ _ _ Hg1hd Hghdtl).
+  Qed.
+
+
+
+  Definition avars_newer_than_var (avn : N) (g : N) (v : ssavar) : Prop :=
+    (svar v != avn) \/ (sidx v < g)%num.
+
+  Definition avars_newer_than (avn : N) (g : N) (vs : SSAVS.t) :=
+    forall v, SSAVS.mem v vs -> avars_newer_than_var avn g v.
+
+
+  Lemma svar_notin_newer_than_singleton avn g v :
+    svar_notin avn (SSAVS.singleton v) -> avars_newer_than_var avn g v.
+  Proof.
+    move=> H. move: (svar_notin_singleton1 H) => {H} H. rewrite /avars_newer_than_var.
+    left; rewrite eq_sym; assumption.
+  Qed.
+
+  Lemma svar_notin_newer_than avn g vs :
+    svar_notin avn vs -> avars_newer_than avn g vs.
+  Proof.
+    move=> H [vn vi] Hv. case Hvn: (vn == avn).
+    - move: (H vi) => Hmem. rewrite -(eqP Hvn) Hv in Hmem. discriminate.
+    - left. move/idP/negP: Hvn. by apply.
+  Qed.
+
+
+  Lemma avars_newer_than_var_le avn g1 g2 v :
+    (g1 <= g2)%num -> avars_newer_than_var avn g1 v ->
+    avars_newer_than_var avn g2 v.
+  Proof.
+    move=> Hle [] Hnew.
+    - left. assumption.
+    - right. exact: (N.lt_le_trans _ _ _ Hnew Hle).
+  Qed.
+
+  Lemma avars_newer_than_le avn g1 g2 vs :
+    (g1 <= g2)%num -> avars_newer_than avn g1 vs ->
+    avars_newer_than avn g2 vs.
+  Proof.
+    move=> Hle Hnew x Hx. move: (Hnew x Hx). exact: (avars_newer_than_var_le Hle).
+  Qed.
+
+  Lemma avars_newer_than_mem avn g1 g2 vs :
+    avars_newer_than avn g1 vs -> SSAVS.mem (avn, g2) vs ->
+    (g2 < g1)%num.
+  Proof.
+    move=> Hnew Hmem. move: (Hnew (avn, g2) Hmem). rewrite /avars_newer_than_var.
+    case => /= H.
+    - rewrite eqxx in H. discriminate.
+    - assumption.
+  Qed.
+
+  Lemma avars_newer_than_empty avn g : avars_newer_than avn g SSAVS.empty.
+  Proof. done. Qed.
+
+  Lemma avars_newer_than_singleton avn g v :
+    avars_newer_than avn g (SSAVS.singleton v) <->
+    avars_newer_than_var avn g v.
+  Proof.
+    split.
+    - move=> Hnew. apply: (Hnew v). apply: SSAVS.Lemmas.mem_singleton2. exact: eqxx.
+    - move=> Hnew x Hmem. move: (SSAVS.Lemmas.mem_singleton1 Hmem) => {Hmem} /eqP Heq.
+      rewrite Heq; assumption.
+  Qed.
+
+  Lemma avars_newer_than_add avn g v vs :
+    avars_newer_than avn g (SSAVS.add v vs) <->
+    (avars_newer_than_var avn g v /\ avars_newer_than avn g vs).
+  Proof.
+    split.
+    - move=> H; split.
+      + exact: (H v (SSAVS.Lemmas.mem_add2 vs (eqxx v))).
+      + move=> x Hx. move: (SSAVS.Lemmas.mem_add3 v Hx) => Hmem. exact: (H x Hmem).
+    - move=> [Hv Hvs] x Hx. case/SSAVS.Lemmas.mem_add1: Hx.
+      + move=> Hxv. rewrite (eqP Hxv). assumption.
+      + move=> Hx. exact: (Hvs x Hx).
+  Qed.
+
+  Lemma avars_newer_than_union avn g vs1 vs2 :
+    avars_newer_than avn g (SSAVS.union vs1 vs2) <->
+    (avars_newer_than avn g vs1 /\ avars_newer_than avn g vs2).
+  Proof.
+    split.
+    - move=> Hun; split; move=> x Hx.
+      + exact: (Hun x (SSAVS.Lemmas.mem_union2 vs2 Hx)).
+      + exact: (Hun x (SSAVS.Lemmas.mem_union3 vs1 Hx)).
+    - move=> [H1 H2] x Hx. case/SSAVS.Lemmas.mem_union1: Hx => Hx.
+      + exact: (H1 x Hx).
+      + exact: (H2 x Hx).
+  Qed.
+
+  Lemma avars_newer_than_equal avn g vs1 vs2 :
+    SSAVS.Equal vs1 vs2 -> avars_newer_than avn g vs1 ->
+    avars_newer_than avn g vs2.
+  Proof.
+    move=> Heq Hnew1 v Hmem. apply: Hnew1.
+    move: (SSAVS.Lemmas.P.equal_sym Heq) => {Heq} Heq.
+    exact: (SSAVS.Lemmas.mem_equal Hmem Heq).
+  Qed.
+
+  Lemma avars_newer_than_eqn avn g e :
+    svar_notin avn (vars_bexp e) ->
+    avars_newer_than avn g (vars_zbexp (eqn_bexp e)).
+  Proof.
+    case: e => [e r] /=. move/svar_notin_union => /= [He Hr].
+    exact: (svar_notin_newer_than g He).
+  Qed.
+
+  Lemma avars_newer_than_split_eqn avn g e :
+    svar_notin avn (vars_bexp e) ->
+    avars_newer_than avn g (vars_zbexp (eands (split_eand (eqn_bexp e)))).
+  Proof.
+    move=> Hni.
+    apply: (avars_newer_than_equal
+              (SSAVS.Lemmas.P.equal_sym (vars_eands_split_eand (eqn_bexp e)))).
+    exact: (avars_newer_than_eqn g).
+  Qed.
+
+  Lemma new_svar_newer_than vs g : avars_newer_than (new_svar vs) g vs.
+  Proof.
+    exact: (svar_notin_newer_than g (new_svar_notin vs)).
+  Qed.
+
+
+  Ltac split_avars_newer_than :=
+    match goal with
+    | |- avars_newer_than _ _ (SSAVS.union _ _) =>
+      apply/avars_newer_than_union; split
+    end.
+
+  Ltac solve_avars_newer_than :=
+    match goal with
+    | |- avars_newer_than _ _ (SSAVS.singleton _) =>
+      apply/avars_newer_than_singleton; solve_avars_newer_than
+    | |- avars_newer_than _ _ (vars_zbexp (eands (carry_constr ?c))) =>
+      apply: (avars_newer_than_equal
+                (SSAVS.Lemmas.P.equal_sym (vars_carry_constr c)));
+      case: (add_carry_constraints options); solve_avars_newer_than
+    | H : is_true (?avn != Var.svar ?t) |- avars_newer_than_var ?avn _ ?t =>
+      left; rewrite eq_sym; assumption
+    | H : svar_notin ?avn (vars_atomic ?a) |-
+      avars_newer_than ?avn ?g (vars_zexp (bv2z_atomic ?a)) =>
+      rewrite vars_bv2z_atomic; exact: (svar_notin_newer_than g H)
+    | |- avars_newer_than _ _ SSAVS.empty =>
+      exact: avars_newer_than_empty
+    | |- avars_newer_than_var _ (N.succ ?g) (_, ?g) =>
+      right; exact: N.lt_succ_diag_r
+    end.
+
+  Lemma bv2z_instr_newer_than E avn g1 g2 i zs :
+    bv2z_instr E avn g1 i = (g2, zs) ->
+    svar_notin avn (vars_instr i) ->
+    avars_newer_than avn g2 (vars_zbexp (eands zs)).
+  Proof.
+    move=> H.
+    case: i H => /=;
+
+    try (intros; repeat case_pairs; rewrite /=;
+    repeat case_svar_notin;
+    repeat split_avars_newer_than;
+    solve_avars_newer_than).
+
+    (* bv2z_cast *)
+    intros; repeat case_pairs; rewrite /=;
+    repeat case_svar_notin;
+    repeat split_avars_newer_than.
+    move: H; rewrite /bv2z_cast => H.
+    repeat case_pairs; rewrite /=; repeat split_avars_newer_than;
+    solve_avars_newer_than.
+
+    (* bv2z_vpc *)
+    intros; repeat case_pairs; rewrite /=;
+    repeat case_svar_notin;
+    repeat split_avars_newer_than.
+    move: H; rewrite /bv2z_vpc => H.
+    repeat case_pairs; rewrite /=; repeat split_avars_newer_than;
+    solve_avars_newer_than.
+
+    intros; repeat case_pairs; rewrite /=.
+    exact: (avars_newer_than_split_eqn g2 H0).
+  Qed.
+
+  Lemma bv2z_program_newer_than E avn g1 g2 p zs :
+    bv2z_program E avn g1 p = (g2, zs) ->
+    svar_notin avn (vars_program p) ->
+    avars_newer_than avn g2 (vars_zbexp (eands zs)).
+  Proof.
+    elim: p E g1 g2 zs => [| i p IH] E g1 g2 zs /=.
+    - move=> *; case_pairs. exact: avars_newer_than_empty.
+    - dcase (bv2z_instr E avn g1 i) => [[g_hd zhd] Hhd].
+      dcase (bv2z_program (instr_succ_typenv i E) avn g_hd p) => [[g_tl ztl] Htl].
+      case=> ? ?; subst. move/svar_notin_union=> [Hi Hp].
+      apply: (avars_newer_than_equal
+                (SSAVS.Lemmas.P.equal_sym (vars_eands_cat zhd ztl))).
+      apply/avars_newer_than_union; split.
+      + apply: (avars_newer_than_le (bv2z_program_idx_inc Htl)).
+        exact: (bv2z_instr_newer_than Hhd Hi).
+      + exact: (IH _ _ _ _ Htl Hp).
+  Qed.
+
+End SSA2Algebra.
+
+
+
+(** Split a specification into safety conditions, range specification,
+    and algebraic specification *)
+Section SplitSpec.
+
+  Import SSA.
+
+  Ltac split_disjoint :=
+    match goal with
+    | H : is_true (VSLemmas.disjoint _ (SSAVS.singleton _)) |- _ =>
+      rewrite VSLemmas.disjoint_singleton in H
+    | H : is_true (VSLemmas.disjoint _ (SSAVS.add _ _)) |- _ =>
+      let H1 := fresh "Hdisj" in let H2 := fresh "Hdisj" in
+      rewrite VSLemmas.disjoint_add in H;
+      move/andP: H => [H1 H2]
+    end.
+
+  Ltac simplify_types :=
+    repeat
+    match goal with
+    | H : context f [atyp ?a (SSATE.add ?v (atyp ?a ?E) ?E)] |- _ =>
+      rewrite atyp_add_same in H
+    | |- context f [atyp ?a (SSATE.add ?v (atyp ?a ?E) ?E)] =>
+      rewrite atyp_add_same
+    | H : context f [SSATE.vtyp ?v (SSATE.add ?v ?t ?E)] |- _ =>
+      rewrite (SSATE.vtyp_add_eq (eqxx v)) in H
+    | |- context f [SSATE.vtyp ?v (SSATE.add ?v ?t ?E)] =>
+      rewrite (SSATE.vtyp_add_eq (eqxx v))
+    | H : context f [SSATE.vtyp ?x (SSATE.add ?y _ _)],
+          Hneq : is_true (?x != ?y) |- _ =>
+      rewrite (SSATE.vtyp_add_neq Hneq) in H
+    | Hneq : is_true (?x != ?y) |- context f [SSATE.vtyp ?x (SSATE.add ?y _ _)] =>
+      rewrite (SSATE.vtyp_add_neq Hneq)
+    | Hneq : is_true (?x != ?y),
+      H : context f [SSATE.vtyp ?x (SSATE.add ?y _ _)] |- _ =>
+      rewrite (SSATE.vtyp_add_neq Hneq) in H
+    | Hmem : is_true (~~ SSAVS.mem ?v (vars_env ?E)),
+      Hsub : is_true (SSAVS.subset (vars_atomic ?a) (vars_env ?E))
+      |- context f [atyp ?a (SSATE.add ?v ?t _)] =>
+      rewrite (atyp_add_not_mem _ _ (SSAVS.Lemmas.not_mem_subset Hmem Hsub))
+    | Hmem : is_true (~~ SSAVS.mem ?v (vars_env ?E)),
+      Hsub : is_true (SSAVS.subset (vars_atomic ?a) (vars_env ?E)),
+      H : context f [atyp ?a (SSATE.add ?v ?t _)] |- _ =>
+      rewrite (atyp_add_not_mem _ _ (SSAVS.Lemmas.not_mem_subset Hmem Hsub)) in H
+    end.
+
+  Ltac defined_dec :=
+    match goal with
+    | H : is_true (are_defined ?vs ?E) |-
+      is_true (are_defined ?vs (SSATE.add _ _ (SSATE.add _ _ ?E))) =>
+      apply: are_defined_addr; apply: are_defined_addr; exact: H
+    | H : is_true (are_defined ?vs ?E) |-
+      is_true (are_defined ?vs (SSATE.add _ _ ?E)) =>
+      apply: are_defined_addr; exact: H
+    end.
+
+  Ltac ssa_vars_unchanged_instr_to_mem :=
+    match goal with
+    | H : is_true (ssa_vars_unchanged_instr ?vs ?i) |- _ =>
+      let Hdisj := fresh "Hdisj" in
+      (have: (ssa_vars_unchanged_instr vs i) by assumption);
+      (rewrite ssa_unchanged_instr_disjoint_lvs => /= Hdisj);
+      repeat split_disjoint
+    end.
+
+  (* State equivalence. *)
+
+  Definition bvz_eq (E : SSATE.env) (sb : SSAStore.t) (sz : ZSSAStore.t) : Prop :=
+    forall x, acc2z E x sb = ZSSAStore.acc x sz.
+
+  Lemma bvz_eq_upd E v bv zv sb sz :
+    bvz_eq E sb sz -> bv2z (SSATE.vtyp v E) bv = zv ->
+    bvz_eq E (SSAStore.upd v bv sb) (ZSSAStore.upd v zv sz).
+  Proof.
+    move=> Heq Hbv x. case Hxv: (x == v).
+    - rewrite (acc2z_upd_eq Hxv) (ZSSAStore.acc_upd_eq Hxv) (eqP Hxv). exact: Hbv.
+    - move/idP/negP: Hxv => Hxv.
+      rewrite (acc2z_upd_neq Hxv) (ZSSAStore.acc_upd_neq Hxv). exact: (Heq x).
+  Qed.
+
+  Lemma bvz_eq_upd2 E vh vl bvh bvl zvh zvl sb sz :
+    bvz_eq E sb sz ->
+    bv2z (SSATE.vtyp vh E) bvh = zvh -> bv2z (SSATE.vtyp vl E) bvl = zvl ->
+    bvz_eq E (SSAStore.upd2 vh bvh vl bvl sb) (ZSSAStore.upd2 vh zvh vl zvl sz).
+  Proof.
+    move=> Heq Hbvh Hbvl x. case Hxvl: (x == vl).
+    - rewrite (acc2z_upd_eq Hxvl) (ZSSAStore.acc_upd_eq Hxvl) (eqP Hxvl). exact: Hbvl.
+    - move/idP/negP: Hxvl => Hxvl.
+      rewrite (acc2z_upd_neq Hxvl) (ZSSAStore.acc_upd_neq Hxvl). case Hxvh: (x == vh).
+      + rewrite (acc2z_upd_eq Hxvh) (ZSSAStore.acc_upd_eq Hxvh) (eqP Hxvh).
+        exact: Hbvh.
+      + move/idP/negP: Hxvh => Hxvh.
+        rewrite (acc2z_upd_neq Hxvh) (ZSSAStore.acc_upd_neq Hxvh). exact: (Heq x).
+  Qed.
+
+  Lemma bvz_eq_eval_atomic a E bs zs :
+    bvz_eq E bs zs ->
+    ZSSA.eval_zexp (bv2z_atomic a) zs = bv2z (atyp a E) (eval_atomic a bs).
+  Proof.
+    move=> Heq. case: a => /=.
+    - move=> v. rewrite -Heq. reflexivity.
+    - move=> t b. reflexivity.
+  Qed.
+
+
+
+  (* State equivalence except newly introduced variables. *)
+
+  Definition bvz_eqm (E : SSATE.env) (tmp : VarOrder.t)
+             (sb : SSAStore.t) (sz : ZSSAStore.t) : Prop :=
+    forall x, tmp != svar x -> acc2z E x sb = ZSSAStore.acc x sz.
+
+  Lemma bvz_eq_eqm E tmp sb sz : bvz_eq E sb sz -> bvz_eqm E tmp sb sz.
+  Proof. move=> H x _. exact: H. Qed.
+
+  Lemma bvz_eqm_upd E v bv zv tmp sb sz :
+    bvz_eqm E tmp sb sz -> bv2z (SSATE.vtyp v E) bv = zv ->
+    bvz_eqm E tmp (SSAStore.upd v bv sb) (ZSSAStore.upd v zv sz).
+  Proof.
+    move=> Heq Hbv x Hne. case Hxv: (x == v).
+    - rewrite (acc2z_upd_eq Hxv) (ZSSAStore.acc_upd_eq Hxv) (eqP Hxv). exact: Hbv.
+    - move/idP/negP: Hxv => Hxv.
+      rewrite (acc2z_upd_neq Hxv) (ZSSAStore.acc_upd_neq Hxv). exact: (Heq _ Hne).
+  Qed.
+
+  Lemma bvz_eqm_upd2 E vh vl bvh bvl zvh zvl tmp sb sz :
+    bvz_eqm E tmp sb sz ->
+    bv2z (SSATE.vtyp vh E) bvh = zvh -> bv2z (SSATE.vtyp vl E) bvl = zvl ->
+    bvz_eqm E tmp (SSAStore.upd2 vh bvh vl bvl sb) (ZSSAStore.upd2 vh zvh vl zvl sz).
+  Proof.
+    move=> Heq Hbvh Hbvl x Hne. case Hxvl: (x == vl).
+    - rewrite (acc2z_upd_eq Hxvl) (ZSSAStore.acc_upd_eq Hxvl) (eqP Hxvl). exact: Hbvl.
+    - move/idP/negP: Hxvl => Hxvl.
+      rewrite (acc2z_upd_neq Hxvl) (ZSSAStore.acc_upd_neq Hxvl). case Hxvh: (x == vh).
+      + rewrite (acc2z_upd_eq Hxvh) (ZSSAStore.acc_upd_eq Hxvh) (eqP Hxvh).
+        exact: Hbvh.
+      + move/idP/negP: Hxvh => Hxvh.
+        rewrite (acc2z_upd_neq Hxvh) (ZSSAStore.acc_upd_neq Hxvh). exact: (Heq _ Hne).
+  Qed.
+
+  Lemma bvz_eqm_upd2_aux E c v bvc bvv zvc zvv zvt tmp idx sb sz :
+  bvz_eqm E tmp sb sz ->
+  bv2z (SSATE.vtyp c E) bvc = zvc -> bv2z (SSATE.vtyp v E) bvv = zvv ->
+    tmp != svar c -> tmp != svar v ->
+    bvz_eqm E tmp
+            (SSAStore.upd2 v bvv c bvc sb)
+            (ZSSAStore.upd c
+                           zvc
+                           (ZSSAStore.upd2 v zvv (tmp, idx) zvt sz)).
+  Proof.
+    move=> Heqm Hc Hv Hnec Hnev x Hnex. case Hxc: (x == c).
+    - rewrite (acc2z_upd2_eq2 Hxc) (ZSSAStore.acc_upd2_eq2 Hxc) (eqP Hxc). exact: Hc.
+    - move/idP/negP: Hxc => Hxc. rewrite (ZSSAStore.acc_upd_neq Hxc).
+      have Hxtmp: x != (tmp, idx).
+      { apply/negP => Heq. move/negP: Hnex; apply. by rewrite (eqP Heq). }
+      case Hxv: (x == v).
+      + rewrite (acc2z_upd2_eq1 Hxv Hxc) (ZSSAStore.acc_upd2_eq1 Hxv Hxtmp) (eqP Hxv).
+        exact: Hv.
+      + move/idP/negP: Hxv => Hxv.
+        rewrite (acc2z_upd2_neq Hxv Hxc) (ZSSAStore.acc_upd2_neq Hxv Hxtmp).
+        exact: (Heqm _ Hnex).
+  Qed.
+
+
+  (* State equivalence considering only variables in an environment. *)
+
+  Definition bvz_eqi (E : SSATE.env) (sb : SSAStore.t) (sz : ZSSAStore.t) : Prop :=
+    forall x, SSATE.mem x E -> acc2z E x sb = ZSSAStore.acc x sz.
+
+  Lemma bvz_eq_eqi E sb sz : bvz_eq E sb sz -> bvz_eqi E sb sz.
+  Proof. move=> Heq x _. exact: (Heq x). Qed.
+
+  Lemma bvz_eqi_upd E v bv zv sb sz :
+    bvz_eqi E sb sz -> bv2z (SSATE.vtyp v E) bv = zv ->
+    bvz_eqi E (SSAStore.upd v bv sb) (ZSSAStore.upd v zv sz).
+  Proof.
+    move=> Heq Hbv x Hx. case Hxv: (x == v).
+    - rewrite (acc2z_upd_eq Hxv) (ZSSAStore.acc_upd_eq Hxv) (eqP Hxv). exact: Hbv.
+    - move/idP/negP: Hxv => Hxv.
+      rewrite (acc2z_upd_neq Hxv) (ZSSAStore.acc_upd_neq Hxv). exact: (Heq x).
+  Qed.
+
+  Lemma bvz_eqi_upd2 E vh vl bvh bvl zvh zvl sb sz :
+    bvz_eqi E sb sz ->
+    bv2z (SSATE.vtyp vh E) bvh = zvh -> bv2z (SSATE.vtyp vl E) bvl = zvl ->
+    bvz_eqi E (SSAStore.upd2 vh bvh vl bvl sb) (ZSSAStore.upd2 vh zvh vl zvl sz).
+  Proof.
+    move=> Heq Hbvh Hbvl x Hx. case Hxvl: (x == vl).
+    - rewrite (acc2z_upd_eq Hxvl) (ZSSAStore.acc_upd_eq Hxvl) (eqP Hxvl). exact: Hbvl.
+    - move/idP/negP: Hxvl => Hxvl.
+      rewrite (acc2z_upd_neq Hxvl) (ZSSAStore.acc_upd_neq Hxvl). case Hxvh: (x == vh).
+      + rewrite (acc2z_upd_eq Hxvh) (ZSSAStore.acc_upd_eq Hxvh) (eqP Hxvh).
+        exact: Hbvh.
+      + move/idP/negP: Hxvh => Hxvh.
+        rewrite (acc2z_upd_neq Hxvh) (ZSSAStore.acc_upd_neq Hxvh). exact: (Heq x).
+  Qed.
+
+  Lemma bvz_eqi_eval_atomic a E bs zs :
+    bvz_eqi E bs zs -> are_defined (vars_atomic a) E ->
+    ZSSA.eval_zexp (bv2z_atomic a) zs = bv2z (atyp a E) (eval_atomic a bs).
+  Proof.
+    move=> Heq. case: a => /=.
+    - move=> v; rewrite are_defined_singleton=> Hdef. rewrite -Heq; first reflexivity.
+      exact: Hdef.
+    - move=> t b _. reflexivity.
+  Qed.
+
+  Lemma bvz_eqi_eval_eexp E e bs zs :
+    bvz_eqi E bs zs -> are_defined (ZSSA.vars_zexp e) E ->
+    eval_eexp e E bs = ZSSA.eval_zexp e zs.
+  Proof.
+    move=> Heq. elim: e => //=.
+    - move=> x; rewrite are_defined_singleton=> Hdef. exact: (Heq x Hdef).
+    - move=> op e IH Hdef. rewrite (IH Hdef). reflexivity.
+    - move=> op e1 IH1 e2 IH2. rewrite are_defined_union=> /andP [Hdef1 Hdef2].
+      rewrite (IH1 Hdef1) (IH2 Hdef2). reflexivity.
+  Qed.
+
+  Lemma bvz_eqi_eval_ebexp E e bs zs :
+    bvz_eqi E bs zs -> are_defined (vars_ebexp e) E ->
+    eval_ebexp e E bs <-> ZSSA.eval_zbexp (eands (split_eand e)) zs.
+  Proof.
+    move=> Heq. elim: e => //=.
+    - move=> e1 e2. rewrite are_defined_union => /andP [Hdef1 Hdef2].
+      rewrite (bvz_eqi_eval_eexp Heq Hdef1) (bvz_eqi_eval_eexp Heq Hdef2). tauto.
+    - move=> e1 e2 e3.
+      rewrite !are_defined_union => /andP [Hdef1 /andP [Hdef2 Hdef3]].
+      rewrite (bvz_eqi_eval_eexp Heq Hdef1) (bvz_eqi_eval_eexp Heq Hdef2)
+              (bvz_eqi_eval_eexp Heq Hdef3). tauto.
+    - move=> e1 IH1 e2 IH2. rewrite are_defined_union => /andP [Hdef1 Hdef2].
+      move: (IH1 Hdef1) (IH2 Hdef2) => H1 H2. split.
+      + move=> [He1 He2]. apply/ZSSA.eval_zbexp_eands_cat. tauto.
+      + move/ZSSA.eval_zbexp_eands_cat=> [He1 He2]. tauto.
+  Qed.
+
+  Lemma submap_bvz_eqi E1 E2 bs zs :
+    TELemmas.submap E1 E2 -> bvz_eqi E2 bs zs -> bvz_eqi E1 bs zs.
+  Proof.
+    move=> Hsub Heqi x Hx. move/defmemP: Hx => Hx.
+    move: (TELemmas.submap_mem Hsub Hx) => Hx2. rewrite -(Heqi x Hx2).
+    exact: (submap_acc2z Hsub Hx).
+  Qed.
+
+
+  (* Convert bit-vector stores to integer stores. *)
+
+  Definition bv2z_store (E : SSATE.env) (bs : SSAStore.t) : ZSSAStore.t :=
+    fun v => acc2z E v bs.
+
+  Lemma acc_bv2z_store E v bs : ZSSAStore.acc v (bv2z_store E bs) = acc2z E v bs.
+  Proof. reflexivity. Qed.
+
+  Lemma bv2z_store_eq E bs : bvz_eq E bs (bv2z_store E bs).
+  Proof. move=> x; reflexivity. Qed.
+
+  Lemma bv2z_store_eqi E bs : bvz_eqi E bs (bv2z_store E bs).
+  Proof. move=> x _. reflexivity. Qed.
+
+  Lemma bvs_bvz_eqi E bs1 bs2 zs :
+    bvs_eqi E bs1 bs2 -> bvz_eqi E bs1 zs -> bvz_eqi E bs2 zs.
+  Proof.
+    move=> Hseq Hzeq x Hx. rewrite -(Hzeq x Hx) /acc2z.
+    rewrite (Hseq x Hx). reflexivity.
+  Qed.
+
+  Lemma bvz_bvs_eqi E bs1 bs2 zs :
+    SSAStore.conform bs1 E -> SSAStore.conform bs2 E ->
+    bvz_eqi E bs1 zs -> bvz_eqi E bs2 zs -> bvs_eqi E bs1 bs2.
+  Proof.
+    move=> Hcon1 Hcon2 Hzeq1 Hzeq2 x Hx. move: (Hzeq1 x Hx) (Hzeq2 x Hx).
+    rewrite /acc2z /bv2z. case: (SSATE.vtyp x E) => wx.
+    - move=> H1 H2; rewrite -H2 in H1.
+      move: (Hcon1 x Hx) (Hcon2 x Hx) => Hs1 Hs2; rewrite Hs1 in Hs2.
+      exact: (to_Zpos_inj_ss Hs2 H1).
+    - move=> H1 H2; rewrite -H2 in H1.
+      move: (Hcon1 x Hx) (Hcon2 x Hx) => Hs1 Hs2; rewrite Hs1 in Hs2.
+      exact: (to_Z_inj_ss Hs2 H1).
+  Qed.
+
+
+  (* Assign auxiliary variables *)
+
+  Definition bv2z_upd_avars_cast
+             (avn : VarOrder.t) (g : N) (v : SSAVarOrder.t) vtyp a atyp
+             (zs : ZSSAStore.t) : N * ZSSAStore.t :=
+    match vtyp, atyp with
+    | Tuint wv, Tuint wa =>
+      if wv >= wa then
+        (g, zs)
+      else
+        let discarded := (avn, g) in
+        let g' := N.succ g in
+        let (q, r) := Z.div_eucl (ZSSA.eval_zexp (bv2z_atomic a) zs)
+                                 (z2expn (Z.of_nat wv)) in
+        let zs' := ZSSAStore.upd discarded q zs in
+        (g', zs')
+    | Tuint wv, Tsint wa =>
+      (* a_sign and discarded have different meanings but
+         the polynomial equation is equivalent. *)
+      (*if wv >= wa then
+        let a_sign := (avn, g) in
+        let g' := N.succ g in
+        let (q, r) := Z.div_eucl (ZSSA.eval_zexp (bv2z_atomic a) zs)
+                                 (z2expn (Z.of_nat wv)) in
+        let zs' := ZSSAStore.upd a_sign q zs in
+        (g', zs')
+      else*)
+        let discarded := (avn, g) in
+        let g' := N.succ g in
+        let (q, r) := Z.div_eucl (ZSSA.eval_zexp (bv2z_atomic a) zs)
+                                 (z2expn (Z.of_nat wv)) in
+        let zs' := ZSSAStore.upd discarded q zs in
+        (g', zs')
+    | Tsint wv, Tuint wa =>
+      if wv > wa then
+        (g, zs)
+      else
+        let discarded := (avn, g) in
+        let g' := N.succ g in
+        let (q, r) := Z.div_eucl (ZSSA.eval_zexp (bv2z_atomic a) zs)
+                                 (z2expn (Z.of_nat wv)) in
+        let zs' := ZSSAStore.upd discarded q zs in
+        (g', zs')
+    | Tsint wv, Tsint wa =>
+      if wv >= wa then
+        (g, zs)
+      else
+        let discarded := (avn, g) in
+        let g' := N.succ g in
+        let (q, r) := Z.div_eucl (ZSSA.eval_zexp (bv2z_atomic a) zs)
+                                 (z2expn (Z.of_nat wv)) in
+        let zs' := ZSSAStore.upd discarded q zs in
+        (g', zs')
+    end.
+
+  Definition bv2z_upd_avars_instr
+             (E : SSATE.env) (avn : VarOrder.t) (g : N) (i : instr)
+             (zs : ZSSAStore.t) : N * ZSSAStore.t :=
+    match i with
+    | Imov v a => (g, zs)
+    | Ishl v a n => (g, zs)
+    | Icshl vh vl a1 a2 n => (g, zs)
+    | Inondet v t => (g, zs)
+    | Icmov v c a1 a2 => (g, zs)
+    | Inop => (g, zs)
+    | Inot v t a => (g, zs)
+    | Iadd v a1 a2 => (g, zs)
+    | Iadds c v a1 a2 => (g, zs)
+    | Iadc v a1 a2 y => (g, zs)
+    | Iadcs c v a1 a2 y => (g, zs)
+    | Isub v a1 a2 => (g, zs)
+    | Isubc c v a1 a2 => (g, zs)
+    | Isubb c v a1 a2 => (g, zs)
+    | Isbc v a1 a2 y => (g, zs)
+    | Isbcs c v a1 a2 y => (g, zs)
+    | Isbb v a1 a2 y => (g, zs)
+    | Isbbs c v a1 a2 y => (g, zs)
+    | Imul v a1 a2 => (g, zs)
+    | Imull vh vl a1 a2 => (g, zs)
+    | Imulj v a1 a2 => (g, zs)
+    | Isplit vh vl a n => (g, zs)
+    | Iand v t a1 a2 => (g, zs)
+    | Ior v t a1 a2 => (g, zs)
+    | Ixor v t a1 a2 => (g, zs)
+    | Icast v t a => bv2z_upd_avars_cast avn g v t a (atyp a E) zs
+    | Ivpc v t a => (g, zs)
+    | Ijoin v ah al => (g, zs)
+    | Iassume e => (g, zs)
+    end.
+
+  Fixpoint bv2z_upd_avars_program
+             (E : SSATE.env) (avn : VarOrder.t) (g : N) (p : program)
+             (zs : ZSSAStore.t) : N * ZSSAStore.t :=
+    match p with
+    | [::] => (g, zs)
+    | hd::tl =>
+      let (g_hd, zs_hd) := bv2z_upd_avars_instr E avn g hd zs in
+      let (g_tl, zs_tl) := bv2z_upd_avars_program
+                             (instr_succ_typenv hd E) avn g_hd tl zs_hd in
+      (g_tl, zs_tl)
+    end.
+
+  Definition bv2z_upd_avars
+             (E : SSATE.env) (avn : VarOrder.t) (g : N) (p : program)
+             (zs : ZSSAStore.t) : ZSSAStore.t :=
+    snd (bv2z_upd_avars_program E avn g p zs).
+
+
+  Lemma bv2z_upd_avars_instr_eqn E avn g i zs :
+    bv2z_upd_avars_instr E avn g (eqn_instr i) zs =
+    bv2z_upd_avars_instr E avn g i zs.
+  Proof. case: i => //=. move=> [] e r /=. reflexivity. Qed.
+
+  Lemma bv2z_upd_avars_program_eqn E avn g p zs :
+    bv2z_upd_avars_program E avn g (eqn_program p) zs =
+    bv2z_upd_avars_program E avn g p zs.
+  Proof.
+    elim: p E g zs => [| i p IH E g zs] //=.
+    dcase (bv2z_upd_avars_instr E avn g (eqn_instr i) zs) => [[g_hde zs_hde] Hhde].
+    dcase (bv2z_upd_avars_program
+             (instr_succ_typenv (eqn_instr i) E) avn g_hde (eqn_program p) zs_hde) =>
+    [[g_tle zs_tle] Htle].
+    rewrite bv2z_upd_avars_instr_eqn in Hhde. rewrite IH eqn_instr_succ_typenv in Htle.
+    rewrite Hhde Htle. reflexivity.
+  Qed.
+
+  Corollary bv2z_upd_avars_eqn E avn g p zs :
+    bv2z_upd_avars E avn g (eqn_program p) zs = bv2z_upd_avars E avn g p zs.
+  Proof.
+    rewrite /bv2z_upd_avars bv2z_upd_avars_program_eqn. reflexivity.
+  Qed.
+
+
+  Lemma bv2z_upd_avars_cast_gen avn g1 v tv a ta g2 g3 zs zs1 zs2 :
+    bv2z_cast avn g1 v tv a ta = (g2, zs) ->
+    bv2z_upd_avars_cast avn g1 v tv a ta zs1 = (g3, zs2) ->
+    g2 = g3.
+  Proof.
+    rewrite /bv2z_cast /bv2z_upd_avars_cast. case: tv => n.
+    - dcase (Z.div_eucl (ZSSA.eval_zexp (bv2z_atomic a) zs1) (z2expn (Z.of_nat n)))
+      => [[q r] H]. case: ta => m; case: (m <= n).
+      + intros; repeat case_pairs. reflexivity.
+      + intros; repeat case_pairs. reflexivity.
+      + intros; repeat case_pairs. reflexivity.
+      + intros; repeat case_pairs. reflexivity.
+    - dcase (Z.div_eucl (ZSSA.eval_zexp (bv2z_atomic a) zs1) (z2expn (Z.of_nat n)))
+      => [[q r] H]. case: ta => m.
+      + case: (m < n).
+        * intros; repeat case_pairs. reflexivity.
+        * intros; repeat case_pairs. reflexivity.
+      + case: (m <= n).
+        * intros; repeat case_pairs. reflexivity.
+        * intros; repeat case_pairs. reflexivity.
+  Qed.
+
+  Lemma bv2z_upd_avars_instr_gen o E avn i g1 g2 g3 zs zs1 zs2 :
+    bv2z_instr o E avn g1 i = (g2, zs) ->
+    bv2z_upd_avars_instr E avn g1 i zs1 = (g3, zs2) ->
+    g2 = g3.
+  Proof.
+    case: i => /=; intros; repeat case_pairs; try reflexivity.
+    (* bv2z_cast *)
+    - exact: (bv2z_upd_avars_cast_gen H H0).
+    (* bv2z_vpc *)
+    - rewrite /bv2z_vpc in H. repeat case_pairs. reflexivity.
+  Qed.
+
+  Lemma bv2z_upd_avars_program_gen o E avn p g1 g2 g3 zs zs1 zs2 :
+    bv2z_program o E avn g1 p = (g2, zs) ->
+    bv2z_upd_avars_program E avn g1 p zs1 = (g3, zs2) ->
+    g2 = g3.
+  Proof.
+    elim: p E g1 g2 g3 zs zs1 zs2 => [| i p IH] E g1 g2 g3 zs zs1 zs3 /=.
+    - intros; repeat case_pairs. reflexivity.
+    - dcase (bv2z_instr o E avn g1 i) => [[g_hd zhd] Hhd].
+      dcase (bv2z_program o (instr_succ_typenv i E) avn g_hd p) => [[g_tl ztl] Htl].
+      case=> ? ?; subst. dcase (bv2z_upd_avars_instr E avn g1 i zs1) =>
+                         [[bv2z_g_hd bv2z_zs_hd] Hbv2z_hd].
+      dcase (bv2z_upd_avars_program
+               (instr_succ_typenv i E) avn bv2z_g_hd p bv2z_zs_hd) =>
+      [[bv2z_g_tl  bv2z_zs_tl] Hbv2z_tl]. case=> ? ?; subst.
+      rewrite (bv2z_upd_avars_instr_gen Hhd Hbv2z_hd) in Htl.
+      rewrite (IH _ _ _ _ _ _ _ Htl Hbv2z_tl). reflexivity.
+  Qed.
+
+  Lemma bv2z_upd_avars_cast_idx_inc avn g1 v tv a ta g2 zs1 zs2 :
+    bv2z_upd_avars_cast avn g1 v tv a ta zs1 = (g2, zs2) ->
+    (g1 <= g2)%num.
+  Proof.
+    move=> Hupd. move: (Logic.eq_refl (bv2z_cast avn g1 v tv a ta)).
+    move: {2}(bv2z_cast avn g1 v tv a ta) => [g3 zi] Hbvz.
+    move: (bv2z_cast_idx_inc Hbvz) => Hg13.
+    rewrite (bv2z_upd_avars_cast_gen Hbvz Hupd) in Hg13. assumption.
+  Qed.
+
+  Lemma bv2z_upd_avars_instr_idx_inc E avn i g1 g2 zs1 zs2 :
+    bv2z_upd_avars_instr E avn g1 i zs1 = (g2, zs2) ->
+    (g1 <= g2)%num.
+  Proof.
+    move=> Hupd. move: (Logic.eq_refl (bv2z_instr default_options E avn g1 i)).
+    move: {2}(bv2z_instr default_options E avn g1 i) => [g3 zi] Hbvz.
+    move: (bv2z_instr_idx_inc Hbvz) => Hg13.
+    rewrite (bv2z_upd_avars_instr_gen Hbvz Hupd) in Hg13. assumption.
+  Qed.
+
+  Lemma bv2z_upd_avars_program_idx_inc E avn p g1 g2 zs1 zs2 :
+    bv2z_upd_avars_program E avn g1 p zs1 = (g2, zs2) ->
+    (g1 <= g2)%num.
+  Proof.
+    move=> Hupd. move: (Logic.eq_refl (bv2z_program default_options E avn g1 p)).
+    move: {2}(bv2z_program default_options E avn g1 p) => [g3 zp] Hbvz.
+    move: (bv2z_program_idx_inc Hbvz) => Hg13.
+    rewrite (bv2z_upd_avars_program_gen Hbvz Hupd) in Hg13. assumption.
+  Qed.
+
+
+  Lemma bv2z_upd_avars_instr_acc_ne E avn g1 i zs1 g2 zs2 v :
+    svar v != avn -> bv2z_upd_avars_instr E avn g1 i zs1 = (g2, zs2) ->
+    ZSSAStore.acc v zs2 = ZSSAStore.acc v zs1.
+  Proof.
+    Ltac mytac :=
+      (move=> *; match goal with
+                 | H : (_, _) = (_, _) |- _ =>
+                   case: H; move=> ? ?; subst; mytac
+                 | H : is_true (?x != ?y) |-
+                   ZSSAStore.acc ?x (ZSSAStore.upd ?y _ ?zs) = ZSSAStore.acc ?x ?zs =>
+                   exact: (ZSSAStore.acc_upd_neq H)
+                 | |- _ => idtac
+                 end).
+    move=> Hne. case: i => //=; try by mytac.
+    (* Icast *)
+    move=> x xt a Hupd. have: v != (avn, g1).
+    { apply/negP=> Heq. move/negP: Hne; apply. case: v Heq. move=> ? ? /eqP [] -> _.
+      exact: eqxx. } move=> {Hne} Hne. move: Hupd. rewrite /bv2z_upd_avars_cast.
+    case: xt; case: (atyp a E) => /=.
+    - move=> wx wa. case: (wx <= wa); [by mytac |].
+      dcase (Z.div_eucl (ZSSA.eval_zexp (bv2z_atomic a) zs1) (z2expn (Z.of_nat wa))).
+      case; by mytac.
+    - move=> wx wa.
+      dcase (Z.div_eucl (ZSSA.eval_zexp (bv2z_atomic a) zs1) (z2expn (Z.of_nat wa))).
+      case; by mytac.
+    - move=> wx wa. case: (wx < wa); [by mytac |].
+      dcase (Z.div_eucl (ZSSA.eval_zexp (bv2z_atomic a) zs1) (z2expn (Z.of_nat wa))).
+      case; by mytac.
+    - move=> wx wa. case: (wx <= wa); [by mytac |].
+      dcase (Z.div_eucl (ZSSA.eval_zexp (bv2z_atomic a) zs1) (z2expn (Z.of_nat wa))).
+      case; by mytac.
+  Qed.
+
+  Lemma bv2z_upd_avars_program_acc_ne E avn g1 p zs1 g2 zs2 v :
+    svar v != avn -> bv2z_upd_avars_program E avn g1 p zs1 = (g2, zs2) ->
+    ZSSAStore.acc v zs2 = ZSSAStore.acc v zs1.
+  Proof.
+    move=> Hne. elim: p E g1 zs1 g2 zs2 => [| i p IH] E g1 zs1 g2 zs2 /=.
+    - case=> _ ->. reflexivity.
+    - dcase (bv2z_upd_avars_instr E avn g1 i zs1) => [[g_hd zs_hd] Hhd].
+      dcase (bv2z_upd_avars_program (instr_succ_typenv i E) avn g_hd p zs_hd) =>
+      [[g_tl zs_tl] Htl]. case=> _ <-. rewrite (IH _ _ _ _ _ Htl).
+      rewrite (bv2z_upd_avars_instr_acc_ne Hne Hhd). reflexivity.
+  Qed.
+
+  Corollary bv2z_upd_avars_acc_ne {E avn g p zs v} :
+    svar v != avn ->
+    ZSSAStore.acc v (bv2z_upd_avars E avn g p zs) = ZSSAStore.acc v zs.
+  Proof.
+    move=> Hne. rewrite /bv2z_upd_avars. dcase (bv2z_upd_avars_program E avn g p zs).
+    case=> [g' zs'] H. exact: (bv2z_upd_avars_program_acc_ne Hne H).
+  Qed.
+
+  Lemma bv2z_upd_avars_instr_acc_lt E avn g1 i zs1 g2 zs2 v :
+    (sidx v < g1)%num -> bv2z_upd_avars_instr E avn g1 i zs1 = (g2, zs2) ->
+    ZSSAStore.acc v zs2 = ZSSAStore.acc v zs1.
+  Proof.
+    Ltac mytac ::=
+      (move=> *; match goal with
+                 | H : (_, _) = (_, _) |- _ =>
+                   case: H; move=> ? ?; subst; mytac
+                 | H : is_true (?x != ?y) |-
+                   ZSSAStore.acc ?x (ZSSAStore.upd ?y _ ?zs) = ZSSAStore.acc ?x ?zs =>
+                   exact: (ZSSAStore.acc_upd_neq H)
+                 | |- _ => idtac
+                 end).
+    move=> Hlt. case: i => //=; try by mytac.
+    (* Icast *)
+    move=> x xt a Hupd. have: v != (avn, g1).
+    { apply/negP=> Heq. rewrite (eqP Heq) /= in Hlt. exact: (N.lt_irrefl _ Hlt). }
+    move=> {Hlt} Hne. move: Hupd. rewrite /bv2z_upd_avars_cast.
+    case: xt; case: (atyp a E) => /=.
+    - move=> wx wa. case: (wx <= wa); [by mytac |].
+      dcase (Z.div_eucl (ZSSA.eval_zexp (bv2z_atomic a) zs1) (z2expn (Z.of_nat wa))).
+      case; by mytac.
+    - move=> wx wa.
+      dcase (Z.div_eucl (ZSSA.eval_zexp (bv2z_atomic a) zs1) (z2expn (Z.of_nat wa))).
+      case; by mytac.
+    - move=> wx wa. case: (wx < wa); [by mytac |].
+      dcase (Z.div_eucl (ZSSA.eval_zexp (bv2z_atomic a) zs1) (z2expn (Z.of_nat wa))).
+      case; by mytac.
+    - move=> wx wa. case: (wx <= wa); [by mytac |].
+      dcase (Z.div_eucl (ZSSA.eval_zexp (bv2z_atomic a) zs1) (z2expn (Z.of_nat wa))).
+      case; by mytac.
+  Qed.
+
+  Lemma bv2z_upd_avars_program_acc_lt E avn g1 p zs1 g2 zs2 v :
+    (sidx v < g1)%num -> bv2z_upd_avars_program E avn g1 p zs1 = (g2, zs2) ->
+    ZSSAStore.acc v zs2 = ZSSAStore.acc v zs1.
+  Proof.
+    elim: p E g1 zs1 g2 zs2 => [| i p IH] E g1 zs1 g2 zs2 Hlt /=.
+    - case=> _ ->. reflexivity.
+    - dcase (bv2z_upd_avars_instr E avn g1 i zs1) => [[g_hd zs_hd] Hhd].
+      dcase (bv2z_upd_avars_program (instr_succ_typenv i E) avn g_hd p zs_hd) =>
+      [[g_tl zs_tl] Htl]. case=> Hg2 <-.
+      move: (bv2z_upd_avars_instr_idx_inc Hhd) => Hg1.
+      move: (N.lt_le_trans _ _ _ Hlt Hg1) => Hg_hd.
+      rewrite (IH _ _ _ _ _ Hg_hd Htl). exact: (bv2z_upd_avars_instr_acc_lt Hlt Hhd).
+  Qed.
+
+  Corollary bv2z_upd_avars_acc_lt {E avn g p zs v} :
+    (sidx v < g)%num ->
+    ZSSAStore.acc v (bv2z_upd_avars E avn g p zs) = ZSSAStore.acc v zs.
+  Proof.
+    move=> Hlt. rewrite /bv2z_upd_avars. dcase (bv2z_upd_avars_program E avn g p zs).
+    case=> [g' zs'] H. exact: (bv2z_upd_avars_program_acc_lt Hlt H).
+  Qed.
+
+  Corollary bv2z_upd_avars_instr_acc_newer E avn g1 i zs1 g2 zs2 v :
+    avars_newer_than_var avn g1 v ->
+    bv2z_upd_avars_instr E avn g1 i zs1 = (g2, zs2) ->
+    ZSSAStore.acc v zs2 = ZSSAStore.acc v zs1.
+  Proof.
+    case; [exact: bv2z_upd_avars_instr_acc_ne | exact: bv2z_upd_avars_instr_acc_lt].
+  Qed.
+
+  Corollary bv2z_upd_avars_program_acc_newer E avn g1 p zs1 g2 zs2 v :
+    avars_newer_than_var avn g1 v ->
+    bv2z_upd_avars_program E avn g1 p zs1 = (g2, zs2) ->
+    ZSSAStore.acc v zs2 = ZSSAStore.acc v zs1.
+  Proof.
+    case; [exact: bv2z_upd_avars_program_acc_ne | exact: bv2z_upd_avars_program_acc_lt].
+  Qed.
+
+  Corollary bv2z_upd_avars_acc_newer {E avn g p zs v} :
+    avars_newer_than_var avn g v ->
+    ZSSAStore.acc v (bv2z_upd_avars E avn g p zs) = ZSSAStore.acc v zs.
+  Proof.
+    case; [exact: bv2z_upd_avars_acc_ne | exact: bv2z_upd_avars_acc_lt].
+  Qed.
+
+
+  Lemma bv2z_upd_avars_instr_eval_zexp E avn i g1 g2 zs1 zs2 e :
+    avars_newer_than avn g1 (ZSSA.vars_zexp e) ->
+    bv2z_upd_avars_instr E avn g1 i zs1 = (g2, zs2) ->
+    ZSSA.eval_zexp e zs1 = ZSSA.eval_zexp e zs2.
+  Proof.
+    move=> Hnew Hupd. elim: e Hnew => //=.
+    - move=> v Hnew. move/avars_newer_than_singleton: Hnew => Hnew.
+      rewrite (bv2z_upd_avars_instr_acc_newer Hnew Hupd). reflexivity.
+    - move=> op e IH Hnew. rewrite (IH Hnew). reflexivity.
+    - move=> op e1 IH1 e2 IH2 /avars_newer_than_union [] Hnew1 Hnew2.
+      rewrite (IH1 Hnew1) (IH2 Hnew2). reflexivity.
+  Qed.
+
+  Lemma bv2z_upd_avars_program_eval_zexp E avn p g1 g2 zs1 zs2 e :
+    avars_newer_than avn g1 (ZSSA.vars_zexp e) ->
+    bv2z_upd_avars_program E avn g1 p zs1 = (g2, zs2) ->
+    ZSSA.eval_zexp e zs1 = ZSSA.eval_zexp e zs2.
+  Proof.
+    elim: p E g1 zs1 g2 zs2 => [| i p IH] E g1 zs1 g2 zs2 /=.
+    - move=> Hnew [] ? ?; subst. reflexivity.
+    - move=> Hnew. dcase (bv2z_upd_avars_instr E avn g1 i zs1) => [[g_hd zs_hd] Hhd].
+      dcase (bv2z_upd_avars_program (instr_succ_typenv i E) avn g_hd p zs_hd) =>
+      [[g_tl zs_tl] Htl]. move=> [] ? ?; subst.
+      rewrite -(IH _ _ _ _ _
+                   (avars_newer_than_le (bv2z_upd_avars_instr_idx_inc Hhd) Hnew) Htl).
+      exact: (bv2z_upd_avars_instr_eval_zexp Hnew Hhd).
+  Qed.
+
+  Lemma bv2z_upd_avars_eval_zexp E avn p g zs1 zs2 e :
+    avars_newer_than avn g (ZSSA.vars_zexp e) ->
+    bv2z_upd_avars E avn g p zs1 = zs2 ->
+    ZSSA.eval_zexp e zs1 = ZSSA.eval_zexp e zs2.
+  Proof.
+    rewrite /bv2z_upd_avars. dcase (bv2z_upd_avars_program E avn g p zs1) =>
+                             [[g2 zs2'] Hupd] /=. move=> Hnew ?; subst.
+    exact: (bv2z_upd_avars_program_eval_zexp Hnew Hupd).
+  Qed.
+
+  Lemma bv2z_upd_avars_instr_eval_zbexp E avn i g1 g2 zs1 zs2 e :
+    avars_newer_than avn g1 (ZSSA.vars_zbexp e) ->
+    bv2z_upd_avars_instr E avn g1 i zs1 = (g2, zs2) ->
+    ZSSA.eval_zbexp e zs1 <-> ZSSA.eval_zbexp e zs2.
+  Proof.
+    move=> Hnew Hupd. elim: e Hnew => //=.
+    - move=> e1 e2 /avars_newer_than_union [Hnew1 Hnew2].
+      rewrite (bv2z_upd_avars_instr_eval_zexp Hnew1 Hupd)
+              (bv2z_upd_avars_instr_eval_zexp Hnew2 Hupd). done.
+    - move=> e1 e2 e3
+                /avars_newer_than_union [Hnew1 /avars_newer_than_union [Hnew2 Hnew3]].
+      rewrite (bv2z_upd_avars_instr_eval_zexp Hnew1 Hupd)
+              (bv2z_upd_avars_instr_eval_zexp Hnew2 Hupd)
+              (bv2z_upd_avars_instr_eval_zexp Hnew3 Hupd). done.
+    - move=> e1 IH1 e2 IH2 /avars_newer_than_union [Hnew1 Hnew2].
+      move: (IH1 Hnew1) (IH2 Hnew2) => {IH1 IH2} H1 H2. tauto.
+  Qed.
+
+  Lemma bv2z_upd_avars_program_eval_zbexp E avn p g1 g2 zs1 zs2 e :
+    avars_newer_than avn g1 (ZSSA.vars_zbexp e) ->
+    bv2z_upd_avars_program E avn g1 p zs1 = (g2, zs2) ->
+    ZSSA.eval_zbexp e zs1 <-> ZSSA.eval_zbexp e zs2.
+  Proof.
+    elim: p E g1 zs1 g2 zs2 => [| i p IH] E g1 zs1 g2 zs2 /=.
+    - move=> Hnew [] ? ?; subst. done.
+    - move=> Hnew. dcase (bv2z_upd_avars_instr E avn g1 i zs1) => [[g_hd zs_hd] Hhd].
+      dcase (bv2z_upd_avars_program (instr_succ_typenv i E) avn g_hd p zs_hd) =>
+      [[g_tl zs_tl] Htl]. move=> [] ? ?; subst.
+      move: (bv2z_upd_avars_instr_idx_inc Hhd) => Hg1.
+      move: (avars_newer_than_le Hg1 Hnew) => Hnew_hd.
+      move: (IH _ _ _ _ _ Hnew_hd Htl) => Heval_tl.
+      move: (bv2z_upd_avars_instr_eval_zbexp Hnew Hhd) => Heval_hd. tauto.
+  Qed.
+
+  Lemma bv2z_upd_avars_eval_zbexp E avn p g zs1 zs2 e :
+    avars_newer_than avn g (ZSSA.vars_zbexp e) ->
+    bv2z_upd_avars E avn g p zs1 = zs2 ->
+    ZSSA.eval_zbexp e zs1 <-> ZSSA.eval_zbexp e zs2.
+  Proof.
+    rewrite /bv2z_upd_avars. dcase (bv2z_upd_avars_program E avn g p zs1) =>
+                             [[g2 zs2'] Hupd] /=. move=> Hnew ?; subst.
+    exact: (bv2z_upd_avars_program_eval_zbexp Hnew Hupd).
+  Qed.
+
+
+  Lemma svar_notin_eval_zexp {zs n g avn e} :
+    svar_notin avn (ZSSA.vars_zexp e) ->
+    ZSSA.eval_zexp e (ZSSAStore.upd (avn, g) n zs) = ZSSA.eval_zexp e zs.
+  Proof.
+    elim: e => //=.
+    - move=> [vn vi]. move/svar_notin_singleton1=> Hni.
+      rewrite ZSSAStore.acc_upd_neq; first by reflexivity.
+      apply/negP=> /eqP [] ? ?; subst. move/negP: Hni; apply. exact: eqxx.
+    - move=> op e IH Hni. rewrite (IH Hni). reflexivity.
+    - move=> op e1 IH1 e2 IH2 /svar_notin_union [Hni1 Hni2].
+      rewrite (IH1 Hni1) (IH2 Hni2). reflexivity.
+  Qed.
+
+  Lemma svar_notin_eval_zbexp zs n g avn e :
+    svar_notin avn (ZSSA.vars_zbexp e) ->
+    ZSSA.eval_zbexp e (ZSSAStore.upd (avn, g) n zs) <-> ZSSA.eval_zbexp e zs.
+  Proof.
+    elim: e => //=.
+    - move=> e1 e2 /svar_notin_union [Hni1 Hni2].
+      rewrite (svar_notin_eval_zexp Hni1) (svar_notin_eval_zexp Hni2). done.
+    - move=> e1 e2 e3 /svar_notin_union [Hni1 /svar_notin_union [Hni2 Hni3]].
+      rewrite (svar_notin_eval_zexp Hni1) (svar_notin_eval_zexp Hni2)
+              (svar_notin_eval_zexp Hni3). done.
+    - move=> e1 IH1 e2 IH2 /svar_notin_union [Hni1 Hni2].
+      move: (IH1 Hni1) (IH2 Hni2) => H1 H2. tauto.
+  Qed.
+
+  Lemma svar_notin_bv2z_upd_avars_instr_eval_zexp E avn g1 i zs1 g2 zs2 e :
+    svar_notin avn (ZSSA.vars_zexp e) ->
+    bv2z_upd_avars_instr E avn g1 i zs1 = (g2, zs2) ->
+    ZSSA.eval_zexp e zs2 = ZSSA.eval_zexp e zs1.
+  Proof.
+    case: i => //=; try (intros; case_pairs; reflexivity).
+    move=> v tv a Hni. rewrite /bv2z_upd_avars_cast. case: tv.
+    - move=> wv. dcase (Z.div_eucl (ZSSA.eval_zexp (bv2z_atomic a) zs1)
+                                   (z2expn (Z.of_nat wv))) => [[q r] Hdiv].
+      case: (atyp a E).
+      + move=> wa. case: (wa <= wv).
+        * case=> ? ?; subst. reflexivity.
+        * case=> ? ?; subst. rewrite (svar_notin_eval_zexp Hni). reflexivity.
+      + move=> _. case=> ? ?; subst. rewrite (svar_notin_eval_zexp Hni). reflexivity.
+    - move=> wv. dcase (Z.div_eucl (ZSSA.eval_zexp (bv2z_atomic a) zs1)
+                                   (z2expn (Z.of_nat wv))) => [[q r] Hdiv].
+      case: (atyp a E).
+      + move=> wa. case: (wa < wv).
+        * case=> ? ?; subst. reflexivity.
+        * case=> ? ?; subst. rewrite (svar_notin_eval_zexp Hni). reflexivity.
+      + move=> wa. case: (wa <= wv).
+        * case=> ? ?; subst. reflexivity.
+        * case=> ? ?; subst. rewrite (svar_notin_eval_zexp Hni). reflexivity.
+  Qed.
+
+  Lemma svar_notin_bv2z_upd_avars_program_eval_zexp E avn g1 p zs1 g2 zs2 e :
+    svar_notin avn (ZSSA.vars_zexp e) ->
+    bv2z_upd_avars_program E avn g1 p zs1 = (g2, zs2) ->
+    ZSSA.eval_zexp e zs2 = ZSSA.eval_zexp e zs1.
+  Proof.
+    elim: p E g1 zs1 g2 zs2 => [| i p IH] E g1 zs1 g2 zs2 Hni /=.
+    - case=> ? ?; subst. reflexivity.
+    - dcase (bv2z_upd_avars_instr E avn g1 i zs1) => [[g_hd zs_hd] Hhd].
+      dcase (bv2z_upd_avars_program (instr_succ_typenv i E) avn g_hd p zs_hd) =>
+      [[g_tl zs_tl] Htl]. case=> ? ?; subst. rewrite (IH _ _ _ _ _ Hni Htl).
+      rewrite (svar_notin_bv2z_upd_avars_instr_eval_zexp Hni Hhd). reflexivity.
+  Qed.
+
+
+  Lemma bvz_zs_eqi zs1 zs2 E bs :
+    bvz_eqi E bs zs1 -> ZSSA.zs_eqi (vars_env E) zs1 zs2 ->
+    bvz_eqi E bs zs2.
+  Proof.
+    move=> Hbeq Hzeq x Hx. rewrite (Hbeq x Hx). move/memenvP: Hx => Hx.
+    exact: (Hzeq x Hx).
+  Qed.
+
+  Lemma bv2z_upd_avars_instr_eqi E1 E2 avn g1 i zs1 g2 zs2 :
+    bv2z_upd_avars_instr E1 avn g1 i zs1 = (g2, zs2) ->
+    svar_notin avn (vars_env E2) ->
+    ZSSA.zs_eqi (vars_env E2) zs1 zs2.
+  Proof.
+    case: i => /=; try (move=> *; case_pairs; exact: ZSSA.zs_eqi_refl).
+    (* Icast *)
+    move=> x tx a Hupd Hni.
+    rewrite /bv2z_upd_avars_cast in Hupd;
+      repeat case_pairs; try exact: ZSSA.zs_eqi_refl.
+    - apply: (ZSSA.zs_eqi_upd _ (Hni g1)). exact: ZSSA.zs_eqi_refl.
+    - apply: (ZSSA.zs_eqi_upd _ (Hni g1)). exact: ZSSA.zs_eqi_refl.
+    - apply: (ZSSA.zs_eqi_upd _ (Hni g1)). exact: ZSSA.zs_eqi_refl.
+    - apply: (ZSSA.zs_eqi_upd _ (Hni g1)). exact: ZSSA.zs_eqi_refl.
+  Qed.
+
+  Lemma bv2z_upd_avars_program_eqi E1 E2 avn g1 p zs1 g2 zs2 :
+    svar_notin avn (vars_env E2) ->
+    bv2z_upd_avars_program E1 avn g1 p zs1 = (g2, zs2) ->
+    ZSSA.zs_eqi (vars_env E2) zs1 zs2.
+  Proof.
+    move=> Hni. elim: p E1 g1 g2 zs1 zs2 => [| i p IH] E1 g1 g2 zs1 zs2 /=.
+    - move=> [] ? ?; subst; exact: ZSSA.zs_eqi_refl.
+    - dcase (bv2z_upd_avars_instr E1 avn g1 i zs1) => [[g_hd zs_hd] Hhd].
+      dcase (bv2z_upd_avars_program (instr_succ_typenv i E1) avn g_hd p zs_hd)
+      => [[g_tl zs_tl] Htl]. case=> ? ?; subst.
+      apply: (ZSSA.zs_eqi_trans (bv2z_upd_avars_instr_eqi Hhd Hni)).
+      exact: (IH _ _ _ _ _  Htl).
+  Qed.
+
+
+  (* main theorem *)
+
+  Lemma bv2z_carry_constraint n :
+    size n = 1 -> (to_Zpos n * (to_Zpos n - 1))%Z = 0%Z.
+  Proof. case: n => //. move=> a [] //=. move=> _. by case: a. Qed.
+
+  Lemma bv2z_Ishl t bs n :
+    size bs = sizeof_typ t -> shlBn_safe t bs n ->
+    bv2z t (bs <<# n)%bits = (bv2z t bs * Cryptoline.DSL.z2expn (Z.of_nat n))%Z.
+  Proof.
+  Admitted.
+
+  Lemma bv2z_Icshl th tl bsh bsl n :
+    is_unsigned tl -> compatible th tl ->
+    size bsh = sizeof_typ th -> size bsl = sizeof_typ tl ->
+    cshlBn_safe th bsh bsl n ->
+    (bv2z tl (low (size bsl) ((bsl ++ bsh) <<# n) >># n)%bits +
+     bv2z th (high (size bsh) ((bsl ++ bsh) <<# n)%bits) *
+     Cryptoline.DSL.z2expn (Z.of_nat (size bsl - n)))%Z =
+    (bv2z th bsh * Cryptoline.DSL.z2expn (Z.of_nat (size bsl)) + bv2z tl bsl)%Z.
+  Proof.
+  Admitted.
+
+  Lemma bv2z_Icmov_true t c a1 a2 :
+    size c = 1 ->
+    to_bool c ->
+    bv2z t a1 = (bv2z Tbit c * bv2z t a1 + (1 - bv2z Tbit c) * bv2z t a2)%Z.
+  Proof.
+    move=> Hs Hc. rewrite /bv2z /=.
+    move: (Seqs.singleton_seq Hs) => {Hs} [b Hcb]. subst.
+    rewrite /to_bool /= negb_and in Hc. case/orP: Hc => Hc; last by done.
+    case: b Hc; last by done. move=> _. rewrite !Z.add_0_r /=.
+    by case: t => wt; [case: (to_Zpos a1) | case: (to_Z a1)].
+  Qed.
+
+  Lemma bv2z_Icmov_false t c a1 a2 :
+    size c = 1 ->
+    ~~ to_bool c ->
+    bv2z t a2 = (bv2z Tbit c * bv2z t a1 + (1 - bv2z Tbit c) * bv2z t a2)%Z.
+  Proof.
+    move=> Hs Hc. rewrite /bv2z /=.
+    move: (Seqs.singleton_seq Hs) => {Hs} [b Hcb]. subst.
+    rewrite /to_bool /= in Hc. move/negPn: Hc => /andP [/eqP -> _] /=.
+    by case: t; [case: (to_Zpos a2) | case: (to_Z a2)].
+  Qed.
+
+  Lemma bv2z_Inot_unsigned t bs n :
+    compatible (Tuint n) t -> size bs = sizeof_typ t ->
+    bv2z (Tuint n) (~~# bs)%bits = (z2expn (Z.of_nat n) - Z.one - bv2z t bs)%Z.
+  Proof.
+  Admitted.
+
+  Lemma bv2z_Inot_signed t bs n :
+    compatible (Tsint n) t -> size bs = sizeof_typ t ->
+    bv2z (Tsint n) (~~# bs)%bits = (- bv2z t bs - Z.one)%Z.
+  Proof.
+  Admitted.
+
+  Lemma bv2z_Iadd t bs1 bs2 :
+    size bs1 = sizeof_typ t -> size bs2 = sizeof_typ t ->
+    addB_safe t bs1 bs2 ->
+    bv2z t (bs1 +# bs2)%bits = (bv2z t bs1 + bv2z t bs2)%Z.
+  Proof.
+  Admitted.
+
+  Lemma bv2z_Iadds_unsigned bs1 bs2 n :
+    size bs1 = n -> size bs2 = n ->
+    (bv2z (Tuint n) (bs1 +# bs2)%bits +
+     bv2z Tbit (1) -bits of bool (carry_addB bs1 bs2)%bits *
+                    Cryptoline.DSL.z2expn (Z.of_nat n))%Z =
+    (bv2z (Tuint n) bs1 + bv2z (Tuint n) bs2)%Z.
+  Proof.
+  Admitted.
+
+  Lemma bv2z_Iadds_signed bs1 bs2 n :
+    size bs1 = n -> size bs2 = n ->
+    adds_safe (Tsint n) bs1 bs2 ->
+    bv2z (Tsint n) (bs1 +# bs2)%bits = (bv2z (Tsint n) bs1 + bv2z (Tsint n) bs2)%Z.
+  Proof.
+  Admitted.
+
+  Lemma bv2z_Iadc t bs1 bs2 bsc :
+    size bs1 = sizeof_typ t -> size bs2 = sizeof_typ t -> size bsc = 1 ->
+    adcB_safe t bs1 bs2 bsc ->
+    bv2z t (adcB (to_bool bsc) bs1 bs2).2 =
+    (bv2z t bs1 + bv2z t bs2 + bv2z Tbit bsc)%Z.
+  Proof.
+  Admitted.
+
+  Lemma bv2z_Iadcs_unsigned bs1 bs2 bsc n :
+    size bs1 = n -> size bs2 = n -> size bsc = 1 ->
+    (bv2z (Tuint n) (adcB (to_bool bsc) bs1 bs2).2 +
+     bv2z Tbit (1)-bits of bool
+                        ((adcB (to_bool bsc) bs1 bs2).1)%bits *
+                   Cryptoline.DSL.z2expn (Z.of_nat n))%Z =
+  (bv2z (Tuint n) bs1 + bv2z (Tuint n) bs2 + bv2z Tbit bsc)%Z.
+  Proof.
+  Admitted.
+
+  Lemma bv2z_Iadcs_signed bs1 bs2 bsc n :
+    size bs1 = n -> size bs2 = n -> size bsc = 1 ->
+    adcs_safe (Tsint n) bs1 bs2 bsc ->
+    bv2z (Tsint n) (adcB (to_bool bsc) bs1 bs2).2 =
+    (bv2z (Tsint n) bs1 + bv2z (Tsint n) bs2 + bv2z Tbit bsc)%Z.
+  Proof.
+  Admitted.
+
+  Lemma bv2z_Isub t bs1 bs2 :
+    size bs1 = sizeof_typ t -> size bs2 = sizeof_typ t ->
+    subB_safe t bs1 bs2 ->
+    bv2z t (bs1 -# bs2)%bits = (bv2z t bs1 - bv2z t bs2)%Z.
+  Proof.
+  Admitted.
+
+  Lemma bv2z_Isubc_unsigned bs1 bs2 n :
+    size bs1 = n -> size bs2 = n ->
+    (bv2z (Tuint n) bs1 - bv2z (Tuint n) bs2 +
+     (1 -  bv2z Tbit (1)-bits of bool (carry_addB bs1 (-# bs2))%bits) *
+     Cryptoline.DSL.z2expn (Z.of_nat n))%Z =
+    bv2z (Tuint n) (bs1 +# -# bs2)%bits.
+  Proof.
+  Admitted.
+
+  Lemma bv2z_Isubc_signed bs1 bs2 n :
+    size bs1 = n -> size bs2 = n ->
+    subc_safe (Tsint n) bs1 bs2 ->
+    bv2z (Tsint n) (bs1 +# -# bs2)%bits = (bv2z (Tsint n) bs1 - bv2z (Tsint n) bs2)%Z.
+  Proof.
+  Admitted.
+
+  Lemma bv2z_Isubb_unsigned bs1 bs2 n :
+    size bs1 = n -> size bs2 = n ->
+    (bv2z (Tuint n) bs1 - bv2z (Tuint n) bs2 +
+     bv2z Tbit (1) -bits of bool (borrow_subB bs1 bs2)%bits *
+                    Cryptoline.DSL.z2expn (Z.of_nat n))%Z =
+    bv2z (Tuint n) (bs1 -# bs2)%bits.
+  Proof.
+  Admitted.
+
+  Lemma bv2z_Isubb_signed bs1 bs2 n :
+    size bs1 = n -> size bs2 = n ->
+    subb_safe (Tsint n) bs1 bs2 ->
+    bv2z (Tsint n) (bs1 -# bs2)%bits = (bv2z (Tsint n) bs1 - bv2z (Tsint n) bs2)%Z.
+  Proof.
+  Admitted.
+
+  Lemma bv2z_Isbc t bs1 bs2 bsc :
+    size bs1 = sizeof_typ t -> size bs2 = sizeof_typ t -> size bsc = 1 ->
+    sbcB_safe t bs1 bs2 bsc ->
+    bv2z t (adcB (to_bool bsc) bs1 (~~# bs2)%bits).2 =
+    (bv2z t bs1 - bv2z t bs2 - (1 - bv2z Tbit bsc))%Z.
+  Proof.
+  Admitted.
+
+  Lemma bv2z_Isbcs_unsigned bs1 bs2 bsc n :
+    size bs1 = n -> size bs2 = n -> size bsc = 1 ->
+    (bv2z (Tuint n) bs1 - bv2z (Tuint n) bs2 - (1 - bv2z Tbit bsc) +
+     (1 - bv2z Tbit (1)-bits of bool
+                             ((adcB (to_bool bsc) bs1 (~~# bs2)).1)%bits) *
+     Cryptoline.DSL.z2expn (Z.of_nat n))%Z =
+    bv2z (Tuint n) (adcB (to_bool bsc) bs1 (~~# bs2)%bits).2.
+  Proof.
+  Admitted.
+
+  Lemma bv2z_Isbcs_signed bs1 bs2 bsc n :
+    size bs1 = n -> size bs2 = n -> size bsc = 1 ->
+    sbcs_safe (Tsint n) bs1 bs2 bsc ->
+    bv2z (Tsint n) (adcB (to_bool bsc) bs1 (~~# bs2)%bits).2 =
+    (bv2z (Tsint n) bs1 - bv2z (Tsint n) bs2 - (1 - bv2z Tbit bsc))%Z.
+  Proof.
+  Admitted.
+
+  Lemma bv2z_Isbb t bs1 bs2 bsc :
+    size bs1 = sizeof_typ t -> size bs2 = sizeof_typ t -> size bsc = 1 ->
+    sbbB_safe t bs1 bs2 bsc ->
+    bv2z t (sbbB (to_bool bsc) bs1 bs2).2 =
+    (bv2z t bs1 - bv2z t bs2 - (1 - bv2z Tbit bsc))%Z.
+  Proof.
+  Admitted.
+
+  Lemma bv2z_Isbbs_unsigned bs1 bs2 bsc n :
+    size bs1 = n -> size bs2 = n -> size bsc = 1 ->
+    (bv2z (Tuint n) (sbbB (to_bool bsc) bs1 bs2).2 +
+     - bv2z Tbit (1)-bits of bool ((sbbB (to_bool bsc) bs1 bs2).1)%bits *
+                     Cryptoline.DSL.z2expn (Z.of_nat n))%Z =
+    (bv2z (Tuint n) bs1 - bv2z (Tuint n) bs2 - bv2z Tbit bsc)%Z.
+  Proof.
+  Admitted.
+
+  Lemma bv2z_Isbbs_signed bs1 bs2 bsc n :
+    size bs1 = n -> size bs2 = n -> size bsc = 1 ->
+    sbbs_safe (Tsint n) bs1 bs2 bsc ->
+    bv2z (Tsint n) (sbbB (to_bool bsc) bs1 bs2).2 =
+    (bv2z (Tsint n) bs1 - bv2z (Tsint n) bs2 - bv2z Tbit bsc)%Z.
+  Proof.
+  Admitted.
+
+  Lemma bv2z_Imul t bs1 bs2 :
+    size bs1 = sizeof_typ t -> size bs2 = sizeof_typ t ->
+    mulB_safe t bs1 bs2 ->
+    bv2z t (bs1 *# bs2)%bits = (bv2z t bs1 * bv2z t bs2)%Z.
+  Proof.
+  Admitted.
+
+  Lemma bv2z_Imull t bs1 bs2 :
+    size bs1 = sizeof_typ t ->
+    size bs2 = sizeof_typ t ->
+    (bv2z (unsigned_typ t) (low (size bs2) (full_mul bs1 bs2)) +
+     bv2z t (high (size bs1) (full_mul bs1 bs2)) *
+     Cryptoline.DSL.z2expn (Z.of_nat (size bs2)))%Z =
+    (bv2z t bs1 * bv2z t bs2)%Z.
+  Proof.
+  Admitted.
+
+  Lemma bv2z_Imulj t bs1 bs2 :
+    size bs1 = sizeof_typ t ->
+    size bs2 = sizeof_typ t ->
+    bv2z (double_typ t) (full_mul bs1 bs2) = (bv2z t bs1 * bv2z t bs2)%Z.
+  Proof.
+  Admitted.
+
+  Lemma bv2z_Isplit_unsigned t bs n :
+    size bs = sizeof_typ t ->
+    (bv2z (unsigned_typ t) (bs <<# (size bs - n) >># (size bs - n))%bits +
+     bv2z t (bs >># n)%bits * Cryptoline.DSL.z2expn (Z.of_nat n))%Z = bv2z t bs.
+  Proof.
+  Admitted.
+
+  Lemma bv2z_Isplit_signed t bs n :
+    size bs = sizeof_typ t ->
+    (bv2z (unsigned_typ t) (bs <<# (size bs - n) >># (size bs - n))%bits +
+     bv2z t (sarB n bs) * Cryptoline.DSL.z2expn (Z.of_nat n))%Z = bv2z t bs.
+  Proof.
+  Admitted.
+
+  (* Upcast from unsigned to unsigned*)
+  Lemma bv2z_Icast_uuu wt wa bs :
+    wa <= wt -> size bs = wa ->
+    bv2z (Tuint wt) (tcast bs (Tuint wa) (Tuint wt)) = bv2z (Tuint wa) bs.
+  Proof.
+  Admitted.
+
+  (* Downcast from unsigned to unsigned *)
+  Lemma bv2z_Icast_duu wt wa bs q r :
+    (wa <= wt) = false -> size bs = wa ->
+    Z.div_eucl (to_Zpos bs) (z2expn (Z.of_nat wt)) = (q, r) ->
+    (bv2z (Tuint wt) (tcast bs (Tuint wa) (Tuint wt)) +
+     q * Cryptoline.DSL.z2expn (Z.of_nat wt))%Z = bv2z (Tuint wa) bs.
+  Proof.
+  Admitted.
+
+  (* Upcast from signed to unsigned *)
+  Lemma bv2z_Icast_usu wt wa bs q r :
+    (wa <= wt) = true -> size bs = wa ->
+    Z.div_eucl (to_Z bs) (z2expn (Z.of_nat wt)) = (q, r) ->
+    (bv2z (Tsint wa) bs + q * Cryptoline.DSL.z2expn (Z.of_nat wt))%Z =
+    bv2z (Tuint wt) (tcast bs (Tsint wa) (Tuint wt)).
+  Proof.
+  Admitted.
+
+  (* Downcast from signed to unsigned *)
+  Lemma bv2z_Icast_dsu wt wa bs q r :
+    (wa <= wt) = false -> size bs = wa ->
+    Z.div_eucl (to_Z bs) (z2expn (Z.of_nat wt)) = (q, r) ->
+    (bv2z (Tuint wt) (tcast bs (Tsint wa) (Tuint wt)) +
+     q * Cryptoline.DSL.z2expn (Z.of_nat wt))%Z = bv2z (Tsint wa) bs.
+  Proof.
+  Admitted.
+
+  (* Upcast from unsigned to signed *)
+  Lemma bv2z_Icast_uus wt wa bs :
+    (wa < wt) = true -> size bs = wa ->
+    bv2z (Tsint wt) (tcast bs (Tuint wa) (Tsint wt)) = bv2z (Tuint wa) bs.
+  Proof.
+  Admitted.
+
+  (* Downcast from unsigned to signed *)
+  Lemma bv2z_Icast_dus wt wa bs q r :
+    (wa < wt) = false -> size bs = wa ->
+    Z.div_eucl (to_Zpos bs) (z2expn (Z.of_nat wt)) = (q, r) ->
+    (bv2z (Tsint wt) (tcast bs (Tuint wa) (Tsint wt)) +
+     q * Cryptoline.DSL.z2expn (Z.of_nat wt))%Z = bv2z (Tuint wa) bs.
+  Proof.
+  Admitted.
+
+  (* Upcast from signed to signed *)
+  Lemma bv2z_Icast_uss wt wa bs :
+    (wa <= wt) = true -> size bs = wa ->
+    bv2z (Tsint wt) (tcast bs (Tsint wa) (Tsint wt)) = bv2z (Tsint wa) bs.
+  Proof.
+  Admitted.
+
+  (* Downcast from signed to signed *)
+  Lemma bv2z_Icast_dss wt wa bs q r :
+    (wa <= wt) = false -> size bs = wa ->
+    Z.div_eucl (to_Z bs) (z2expn (Z.of_nat wt)) = (q, r) ->
+    (bv2z (Tsint wt) (tcast bs (Tsint wa) (Tsint wt)) +
+     q * Cryptoline.DSL.z2expn (Z.of_nat wt))%Z = bv2z (Tsint wa) bs.
+  Proof.
+  Admitted.
+
+  Lemma bv2z_Ivpc tv ta bs :
+    size bs = sizeof_typ ta -> vpc_safe tv ta bs ->
+    bv2z tv (tcast bs ta tv) = bv2z ta bs.
+  Proof.
+  Admitted.
+
+  Lemma bv2z_Ijoin th tl bsh bsl :
+    compatible th tl ->
+    size bsh = sizeof_typ th -> size bsl = sizeof_typ tl ->
+    (bv2z tl bsl + bv2z th bsh * Cryptoline.DSL.z2expn (Z.of_nat (size bsl)))%Z =
+    bv2z (double_typ th) (bsl ++ bsh).
+  Proof.
+  Admitted.
+
+
+  Derive Inversion_clear eval_program_cons_inv with
+      (forall E i p s1 s2, eval_program E (i::p) s1 s2) Sort Prop.
+
+  Ltac acc_zs_to_bs :=
+    repeat
+    match goal with
+    | Heq : bvz_eqi (SSATE.add ?v ?t ?E) ?bs ?zs |- context f [ZSSAStore.acc ?v ?zs] =>
+      rewrite -(Heq v (SSATE.Lemmas.mem_add_eq (eqxx v)))
+    | Heq : bvz_eqi (SSATE.add ?vh ?th (SSATE.add ?vl ?tl ?E)) ?bs ?zs,
+      Hneq : is_true (?vh != ?vl) |-
+      context f [ZSSAStore.acc ?vl ?zs] =>
+      let Hneq' := fresh in
+      rewrite -(Heq vl); last by
+      (move: (negP Hneq) => Hneq'; rewrite eq_sym in Hneq';
+      rewrite (SSATE.Lemmas.mem_add_neq Hneq'));
+      exact (SSATE.Lemmas.mem_add_eq (eqxx vl))
+    | Hupd : SSAStore.Upd ?v ?e ?bs1 ?bs2 |- context f [acc2z ?E ?v ?bs2] =>
+      rewrite (acc2z_Upd_eq (eqxx v) Hupd)
+    | Heq : is_true (?x == ?v), Hupd : SSAStore.Upd ?v ?e ?bs1 ?bs2 |-
+      context f [acc2z ?E ?x ?bs2] =>
+      rewrite (acc2z_Upd_eq Heq Hupd)
+    | Hneq : is_true (?x != ?v), Hupd : SSAStore.Upd ?v ?e ?bs1 ?bs2 |-
+      context f [acc2z ?E ?x ?bs2] =>
+      rewrite (acc2z_Upd_neq Hneq Hupd)
+    | Hupd : SSAStore.Upd2 ?vl ?el ?vh ?eh ?bs1 ?bs2 |-
+      context f [acc2z ?E ?vh ?bs2] =>
+      rewrite (acc2z_Upd2_eq2 (eqxx vh) Hupd)
+    | Hneq : is_true (?vh != ?vl), Hupd : SSAStore.Upd2 ?vl ?el ?vh ?eh ?bs1 ?bs2 |-
+      context f [acc2z ?E ?vl ?bs2] =>
+      rewrite eq_sym in Hneq; rewrite (acc2z_Upd2_eq1 (eqxx vl) Hneq Hupd)
+    | Hni : svar_notin ?avn _, Hne : is_true (?avn != Var.svar ?v) |-
+      context f [ZSSAStore.acc ?v (ZSSAStore.upd (?avn, _) _ _)] =>
+      let H := fresh in
+      rewrite ZSSAStore.acc_upd_neq;
+      last by (apply/eqP=> H; rewrite H /= eqxx in Hne; discriminate)
+    | |- context f [ZSSAStore.acc ?v (ZSSAStore.upd ?v _ _)] =>
+      rewrite ZSSAStore.acc_upd_eq; last exact: eqxx
+    end.
+
+  Ltac eval_zs_to_bs :=
+    repeat
+    match goal with
+    | H : svar_notin ?avn (vars_atomic ?a) |-
+      (* remove the update of auxiliary variables *)
+      context f [ZSSAStore.upd (?avn, _) _ ?zs] =>
+      rewrite svar_notin_eval_zexp; last by (rewrite vars_bv2z_atomic; exact: H)
+    | Heq : bvz_eqi (SSATE.add ?v ?t ?E) ?bs ?zs
+      |- context f [ZSSA.eval_zexp (bv2z_atomic ?a) ?zs] =>
+      rewrite (bvz_eqi_eval_atomic Heq); last by defined_dec
+    | Heq : bvz_eqi (SSATE.add ?v ?t ?E) ?bs ?zs,
+      H : context f [ZSSA.eval_zexp (bv2z_atomic ?a) ?zs] |- _ =>
+      rewrite (bvz_eqi_eval_atomic Heq) in H; last by defined_dec
+    end.
+
+  (* rewrite (eval_atomic a bs2) to (eval_atomic a bs1) where bs1 is a
+     predecessor of bs2 *)
+  Ltac eval_atomic_to_prev :=
+    repeat
+    match goal with
+    | Hun : is_true (ssa_vars_unchanged_instr ?vs ?i),
+      Hsub : is_true (SSAVS.subset (vars_atomic ?a) ?vs),
+      Heval : eval_instr ?E ?i ?bs1 ?bs2 |-
+      context f [eval_atomic ?a ?bs2] =>
+      rewrite -(ssa_unchanged_instr_eval_atomic
+                  (ssa_unchanged_instr_subset Hun Hsub) Heval)
+    | Hun : is_true (ssa_vars_unchanged_instr ?vs ?i),
+      Hsub : is_true (SSAVS.subset (vars_atomic ?a) ?vs),
+      Heval : eval_instr ?E ?i ?bs1 ?bs2,
+      H : context f [eval_atomic ?a ?bs2] |- _ =>
+      rewrite -(ssa_unchanged_instr_eval_atomic
+                  (ssa_unchanged_instr_subset Hun Hsub) Heval) in H
+    end.
+
+  (* If the type of an atomic a is Tbit in some typing environment E, and
+     some state s conforms to E, introduce size (eval_atomic a s) = 1. *)
+  Ltac intro_size_carry :=
+    match goal with
+    | Hco : SSAStore.conform ?bs1 ?E,
+      H : is_true (atyp ?c ?E == Tbit),
+      Hsub : is_true (SSAVS.subset (vars_atomic ?c) (vars_env ?E)) |- _ =>
+      let Hsc := fresh "Hsc" in
+      (move: (size_eval_atomic_asize Hsub Hco) => Hsc);
+      rewrite /asize (eqP H) /= in Hsc
+    end.
+
+  (* Unfold well_formed_instr and split all the Boolean conjunction. *)
+  Ltac unfold_well_formed_instr :=
+    match goal with
+    | H : is_true (well_formed_instr _ _) |- _ =>
+      let Hdef := fresh "Hdef" in
+      let Hwt := fresh "Hwt" in
+      move/andP: H=> [Hdef Hwt]; repeat unfold_well_formed_instr
+    | H : is_true (well_defined_instr _ _) |- _ =>
+      rewrite /well_defined_instr in H; hyps_splitb
+    | H : is_true (well_typed_instr _ _) |- _ =>
+      rewrite /well_typed_instr in H; hyps_splitb
+    end.
+
+  (* For each are_defined vs E, introduce SSAVS.subset vs (vars_env E). *)
+  Ltac intro_subset_from_are_defined :=
+    match goal with
+    | H : is_true (are_defined _ _) |- _ =>
+      let Hsub := fresh "Hsub" in
+      move: (H) => /defsubP Hsub; move: H; intro_subset_from_are_defined
+    | |- _ => intros
+    end.
+
+  (* Introduce size (eval_atomic a s) = sizeof_typ (atyp a E) and
+     rewrite asize a E. *)
+  Ltac intro_atomic_size :=
+    match goal with
+    | Hco : SSAStore.conform ?bs ?E,
+      Hsub : is_true (SSAVS.subset (vars_atomic ?a) (vars_env ?E)) |- _ =>
+      let Hsize := fresh "Hsize" in
+      move: (conform_size_eval_atomic Hsub Hco) => Hsize; move: Hsub; intro_atomic_size
+    | |- _ =>
+      intros; try rewrite /asize;
+      repeat (match goal with
+              | H : _ = sizeof_typ (atyp ?a ?E)
+                |- context f [sizeof_typ (atyp ?a ?E)] =>
+                rewrite -H
+              end)
+    end.
+
+  Ltac rewrite_types :=
+    match goal with
+    | H : is_true (atyp _ _ == _) |- _ => move/eqP: H => H; rewrite_types
+    | H : is_true (_ == atyp _ _) |- _ => move/eqP: H => H; rewrite_types
+    | H1 : atyp ?a1 ?E = atyp ?a2 ?E |- _ =>
+      repeat (match goal with
+              | H2 : context f [atyp a2 E] |- _ => rewrite -H1 /= in H2
+              | |- context f [atyp a2 E] => rewrite -H1
+              end); clear H1; rewrite_types
+    | H1 : atyp ?a1 ?E = _ |- _ =>
+      repeat (match goal with
+              | H2 : context f [atyp a1 E] |- _ => rewrite H1 /= in H2
+              | |- context f [atyp a1 E] => rewrite H1
+              end); clear H1; rewrite_types
+    | |- _ => idtac
+    end.
+
+  (* Prove carry_constr. *)
+  Ltac prove_carry_constr :=
+    match goal with
+    | |- context f [carry_constr ?o ?v] =>
+      rewrite /carry_constr; (case: (add_carry_constraints o) => /=; last by trivial);
+      (split; last by trivial); acc_zs_to_bs; simplify_types;
+      exact: bv2z_carry_constraint
+    end.
+
+  Lemma bv2z_upd_avars_sat_instr o E avn i bs1 bs2 g1 g2 g2' zes zs1 zs2 :
+    well_formed_instr E i ->
+    ssa_vars_unchanged_instr (vars_env E) i ->
+    svar_notin avn (vars_instr i) ->
+    SSAStore.conform bs1 E ->
+    ssa_instr_safe_at E i bs1 ->
+    eval_instr E i bs1 bs2 ->
+    bv2z_instr o E avn g1 i = (g2, zes) ->
+    bv2z_upd_avars_instr E avn g1 i zs1 = (g2', zs2) ->
+    bvz_eqi (instr_succ_typenv i E) bs2 zs1 ->
+    ZSSA.eval_zbexp (eands zes) zs2.
+  Proof.
+    Ltac mytac ::=
+      match goal with
+      | Hev : eval_instr _ _ _ _ |- _ =>
+        unfold_well_formed_instr; ssa_vars_unchanged_instr_to_mem;
+        intro_subset_from_are_defined;
+        (* rewrite the RHS *)
+        repeat case_svar_notin; eval_zs_to_bs;
+        eval_atomic_to_prev; simplify_types;
+        (* rewrite the LHS *)
+        inversion_clear Hev; acc_zs_to_bs; simplify_types;
+        (* *)
+        intro_atomic_size; rewrite_types
+      end.
+    case: i => /=.
+    (* Imov *)
+    - move=> v a Hwf Hun Hni Hco _ Hev [] ? ? [] ? ? Heq; subst; rewrite /=.
+      split; last by trivial. mytac. reflexivity.
+    (* Ishl *)
+    - move=> v a n Hwf Hun Hni Hco Hsa Hev [] ? ? [] ? ? Heq; subst; rewrite /=.
+      split; last by trivial. mytac. exact: (bv2z_Ishl Hsize Hsa).
+    (* Icshl *)
+    - move=> vh vl ah al n Hwf Hun Hni Hco Hsa Hev [] ? ? [] ? ? Heq; subst;
+               rewrite /=. split; last by trivial. mytac.
+      exact: (bv2z_Icshl H H3 Hsize0 Hsize Hsa).
+    (* Inondet *)
+    - move=> v t Hwf Hun Hni Hco _ Hev.
+      case Ht: (t == Tbit); (move=> [] ? ? [] ? ? Heq; subst; rewrite /=);
+        last by trivial. ssa_vars_unchanged_instr_to_mem. move/eqP: Ht => ?; subst.
+      inversion_clear Hev. by prove_carry_constr.
+    (* Icmov *)
+    - move=> v c a1 a2 Hwf Hun Hni Hco _ Hev [] ? ? [] ? ? Heq; subst; rewrite /=.
+      split; last by trivial. mytac.
+      + exact: (bv2z_Icmov_true _ _ _ Hsize0 H7).
+      + exact: (bv2z_Icmov_false _ _ _ Hsize0 H7).
+    (* Inop *)
+    - move=> Hwf Hun Hni Hco _ Hev [] ? ? [] ? ? Heq; subst; rewrite /=. done.
+    (* Inot *)
+    - move=> v t a Hwf Hun Hni Hco _ Hev. case: t Hwf Hun Hev => n Hwf Hun Hev.
+      + move=> [] ? ? [] ? ? Heq; subst; rewrite /=. split; last by trivial.
+        mytac. exact: (bv2z_Inot_unsigned Hwt Hsize).
+      + move=> [] ? ? [] ? ? Heq; subst; rewrite /=. split; last by trivial.
+        mytac. exact: (bv2z_Inot_signed Hwt Hsize).
+    (* Iadd *)
+    - move=> v a1 a2 Hwf Hun Hni Hco Hsa Hev [] ? ? [] ? ? Heq; subst. rewrite /=.
+      split; last by trivial. mytac. exact: (bv2z_Iadd Hsize Hsize0 Hsa).
+    (* Iadds *)
+    - move=> y v a1 a2 Hwf Hun Hni Hco Hsa Hev. dcase (atyp a1 E). case => n Hta1.
+      + move=> [] ? ? [] ? ? Heq; subst. rewrite /=. split.
+        * mytac. exact: (bv2z_Iadds_unsigned Hsize0 Hsize).
+        * inversion_clear Hev. by prove_carry_constr.
+      + move=> [] ? ? [] ? ? Heq; subst. rewrite /=. split; last by trivial.
+        mytac. exact: (bv2z_Iadds_signed Hsize0 Hsize Hsa).
+    (* Iadc *)
+    - move=> v a1 a2 ac Hwf Hun Hni Hco Hsa Hev [] ? ? [] ? ? Heq; subst.
+      rewrite /=. split; last by done. mytac.
+      exact: (bv2z_Iadc Hsize0 Hsize1 Hsize Hsa).
+    (* Iadcs *)
+    - move=> c v a1 a2 ac Hwf Hun Hni Hco Hsa Hev. dcase (atyp a1 E). case=> n Hta1.
+      + move=> [] ? ? [] ? ? Heq; subst. rewrite /=. split.
+        * mytac. exact: (bv2z_Iadcs_unsigned Hsize1 Hsize0 Hsize).
+        * inversion_clear Hev. by prove_carry_constr.
+      + move=> [] ? ? [] ? ? Heq; subst. rewrite /=. split; last by done.
+        mytac. exact: (bv2z_Iadcs_signed Hsize1 Hsize0 Hsize Hsa).
+    (* Isub *)
+    - move=> v a1 a2 Hwf Hun Hni Hco Hsa Hev [] ? ? [] ? ? Heq; subst.
+      rewrite /=. split; last by done. mytac. exact: (bv2z_Isub Hsize Hsize0 Hsa).
+    (* Isubc *)
+    - move=> c v a1 a2 Hwf Hun Hni Hco Hsa Hev. dcase (atyp a1 E). case=> n Hta1.
+      + move=> [] ? ? [] ? ? Heq; subst. rewrite /=. split.
+        * mytac. exact: (bv2z_Isubc_unsigned Hsize0 Hsize).
+        * inversion_clear Hev. by prove_carry_constr.
+      + move=> [] ? ? [] ? ? Heq; subst. rewrite /=. split; last by done.
+        mytac. exact: (bv2z_Isubc_signed Hsize0 Hsize Hsa).
+    (* Isubb *)
+    - move=> c v a1 a2 Hwf Hun Hni Hco Hsa Hev. dcase (atyp a1 E). case=> n Hta1.
+      + move=> [] ? ? [] ? ? Heq; subst. rewrite /=. split.
+        * mytac. exact: (bv2z_Isubb_unsigned Hsize0 Hsize).
+        * inversion_clear Hev. by prove_carry_constr.
+      + move=> [] ? ? [] ? ? Heq; subst. rewrite /=. split; last by done.
+        mytac. exact: (bv2z_Isubb_signed Hsize0 Hsize Hsa).
+    (* Isbc *)
+    - move=> v a1 a2 ac Hwf Hun Hni Hco Hsa Hev [] ? ? [] ? ? Heq; subst.
+      rewrite /=. split; last by done. mytac.
+      exact: (bv2z_Isbc Hsize0 Hsize1 Hsize Hsa).
+    (* Isbcs *)
+    - move=> c v a1 a2 ac Hwf Hun Hni Hco Hsa Hev. dcase (atyp a1 E). case=> n Hta1.
+      + move=> [] ? ? [] ? ? Heq; subst. rewrite /=. split.
+        * mytac. exact: (bv2z_Isbcs_unsigned Hsize1 Hsize0 Hsize).
+        * inversion_clear Hev. by prove_carry_constr.
+      + move=> [] ? ? [] ? ? Heq; subst. rewrite /=. split; last by done.
+        mytac. exact: (bv2z_Isbcs_signed Hsize1 Hsize0 Hsize Hsa).
+    (* Isbb *)
+    - move=> v a1 a2 ac Hwf Hun Hni Hco Hsa Hev [] ? ? [] ? ? Heq; subst.
+      rewrite /=. split; last by done. mytac.
+      exact: (bv2z_Isbb Hsize0 Hsize1 Hsize Hsa).
+    (* Isbbs *)
+    - move=> c v a1 a2 ac Hwf Hun Hni Hco Hsa Hev. dcase (atyp a1 E). case=> n Hta1.
+      + move=> [] ? ? [] ? ? Heq; subst. rewrite /=. split.
+        * mytac. exact: (bv2z_Isbbs_unsigned Hsize1 Hsize0 Hsize).
+        * inversion_clear Hev. by prove_carry_constr.
+      + move=> [] ? ? [] ? ? Heq; subst. rewrite /=. split; last by done.
+        mytac. exact: (bv2z_Isbbs_signed Hsize1 Hsize0 Hsize Hsa).
+    (* Imul *)
+    - move=> v a1 a2 Hwf Hun Hni Hco Hsa Hev [] ? ? [] ? ? Heq; subst. rewrite /=.
+      split; last by trivial. mytac. exact: (bv2z_Imul Hsize Hsize0 Hsa).
+    (* Imull *)
+    - move=> vh vl a1 a2 Hwf Hni Hun Hco Hsa Hev [] ? ? [] ? ? Heq; subst. rewrite /=.
+      split; last by trivial. mytac. exact: (bv2z_Imull Hsize0 Hsize).
+    (* Imulj *)
+    - move=> v a1 a2 Hwf Hun Hni Hco Hsa Hev [] ? ? [] ? ? Heq; subst. rewrite /=.
+      split; last by trivial. mytac. exact: (bv2z_Imulj Hsize Hsize0).
+    (* Isplit *)
+    - move=> vh vl a n Hwf Hun Hni Hco Hsa Hev [] ? ? [] ? ? Heq; subst. rewrite /=.
+      split; last by trivial. mytac.
+      + exact: (bv2z_Isplit_unsigned _ Hsize).
+      + exact: (bv2z_Isplit_signed _ Hsize).
+    (* Iand *)
+    - move=> v t a1 a2 Hwf Hun Hni Hco Hsa Hev [] ? ? [] ? ? Heq; subst. done.
+    (* Ior *)
+    - move=> v t a1 a2 Hwf Hun Hni Hco Hsa Hev [] ? ? [] ? ? Heq; subst. done.
+    (* Ixor *)
+    - move=> v t a1 a2 Hwf Hun Hni Hco Hsa Hev [] ? ? [] ? ? Heq; subst. done.
+    (* Icast *)
+    - move=> v t a. rewrite /bv2z_cast /bv2z_upd_avars_cast.
+      case: t => wt; dcase (atyp a E); case => wa Hta Hwf Hun Hni Hco Hsa Hev.
+      + case Hwa: (wa <= wt).
+        * move=> [] ? ? [] ? ? Heq; subst. rewrite /=. split; last by done.
+          mytac. exact: (bv2z_Icast_uuu Hwa Hsize).
+        * move=> [] ? ? H; subst. repeat case_pairs. rewrite /=. split; last by done.
+          mytac. exact: (bv2z_Icast_duu Hwa Hsize H0).
+      + case Hwa: (wa <= wt).
+        * move=> [] ? ? H; subst. repeat case_pairs. rewrite /=. split; last by done.
+          mytac. exact: (bv2z_Icast_usu Hwa Hsize H0).
+        * move=> [] ? ? H; subst. repeat case_pairs. rewrite /=. split; last by done.
+          mytac. exact: (bv2z_Icast_dsu Hwa Hsize H0).
+      + case Hwa: (wa < wt).
+        * move=> [] ? ? [] ? ? Heq; subst. rewrite /=. split; last by done.
+          mytac. exact: (bv2z_Icast_uus Hwa Hsize).
+        * move=> [] ? ? H; subst. repeat case_pairs. rewrite /=. split; last by done.
+          mytac. exact: (bv2z_Icast_dus Hwa Hsize H0).
+      + case Hwa: (wa <= wt).
+        * move=> [] ? ? [] ? ? Heq; subst. rewrite /=. split; last by done.
+          mytac. exact: (bv2z_Icast_uss Hwa Hsize).
+        * move=> [] ? ? H; subst. repeat case_pairs. rewrite /=. split; last by done.
+          mytac. exact: (bv2z_Icast_dss Hwa Hsize H0).
+    (* Ivpc *)
+    - move=> v t a Hwf Hni Hun Hco Hsa Hev [] ? ? [] ? ? Heq; subst. rewrite /=.
+      split; last by trivial. mytac. exact: (bv2z_Ivpc Hsize Hsa).
+    (* Ijoin *)
+    - move=> v a1 a2 Hwf Hni Hun Hco Hsa Hev [] ? ? [] ? ? Heq; subst. rewrite /=.
+      split; last by trivial. mytac. exact: (bv2z_Ijoin H2 Hsize Hsize0).
+    (* Iassume *)
+    - move=> [e r] /= Hwf Hun Hni Hco Hsa Hev [] ? ? [] ? ? Heq; subst.
+      mytac. rewrite are_defined_union /= in Hdef. move/andP: Hdef => [Hdef _].
+      move: H => [/= He _]. apply/(bvz_eqi_eval_ebexp Heq Hdef). exact: He.
+  Qed.
+
+  Lemma bv2z_upd_avars_sat_program o E avn g1 p g2 eprogs bs1 bs2 :
+    well_formed_program E p ->
+    ssa_vars_unchanged_program (vars_env E) p ->
+    ssa_single_assignment p ->
+    svar_notin avn (vars_env E) -> svar_notin avn (vars_program p) ->
+    SSAStore.conform bs1 E ->
+    ssa_program_safe_at E p bs1 ->
+    eval_program E p bs1 bs2 ->
+    bv2z_program o E avn g1 p = (g2, eprogs) ->
+    ZSSA.eval_zbexp (eands eprogs)
+                    (bv2z_upd_avars E avn g1 p
+                                    (bv2z_store (program_succ_typenv p E) bs2)).
+  Proof.
+    rewrite /bv2z_upd_avars. move: (@bv2z_store_eqi (program_succ_typenv p E) bs2).
+    move: (bv2z_store (program_succ_typenv p E) bs2) => zs2.
+
+    elim: p E g1 g2 eprogs bs1 bs2 zs2 =>
+    [| i p IH] E g1 g2 eprogs bs1 bs2 zs2 /= Heqi2 Hwf Hun Hssa
+               Hni_E Hni_p Hco Hsa Hev Hbv2z.
+    - case: Hbv2z => ? ?; subst => /=. by trivial.
+    - move: Hbv2z. inversion Hev using eval_program_cons_inv => {Hev} bs3 Hi Hp.
+      dcase (bv2z_instr o E avn g1 i) => [[g_hd zhd] Hhd].
+      dcase (bv2z_program o (instr_succ_typenv i E) avn g_hd p) => [[g_tl ztl] Htl].
+      case=> ? ?; subst. move/andP: Hwf => [Hwf_i Hwf_p].
+      move/andP: Hssa => [Hssa_i Hssa_p]. rewrite ssa_unchanged_program_cons in Hun.
+      move/andP: Hun=> [Hun_i Hun_p]. move/svar_notin_union: Hni_p => [Hni_i Hni_p].
+      inversion_clear Hsa. move: H H0 => Hsa_i Hsa_p. rewrite /bv2z_upd_avars /=.
+      dcase (bv2z_upd_avars_instr E avn g1 i zs2) => [[g_hd' zs_hd] Hupd_hd].
+      dcase (bv2z_upd_avars_program (instr_succ_typenv i E) avn g_hd' p zs_hd) =>
+      [[g_tl' zs_tl] Hupd_tl].
+      move: (bv2z_upd_avars_instr_gen Hhd Hupd_hd) => ?; subst.
+      move: (bv2z_upd_avars_program_gen Htl Hupd_tl) => ?; subst.
+      rewrite /=.
+
+      have Hun_iep: ssa_vars_unchanged_program (vars_env (instr_succ_typenv i E)) p.
+      { apply: (ssa_unchanged_program_replace
+                  (SSAVS.Lemmas.P.equal_sym (vars_env_instr_succ_typenv i E))).
+          by rewrite ssa_unchanged_program_union Hun_p Hssa_i. }
+
+      have Hni_lvi: svar_notin avn (lvs_instr i).
+      { apply: (svar_notin_subset _ Hni_i). rewrite vars_instr_split.
+        exact: SSAVS.Lemmas.union_subset_1. }
+      have Hni_lvp: svar_notin avn (lvs_program p).
+      { apply: (svar_notin_subset _ Hni_p). rewrite vars_program_split.
+        exact: SSAVS.Lemmas.union_subset_1. }
+
+      have Hni_ie: svar_notin avn (vars_env (instr_succ_typenv i E)).
+      { apply: (svar_notin_replace
+                  (SSAVS.Lemmas.P.equal_sym (vars_env_instr_succ_typenv i E))).
+        apply/svar_notin_union. split; [exact: Hni_E | exact: Hni_lvi]. }
+
+      apply/ZSSA.eval_zbexp_eands_cat. split.
+      + apply/(bv2z_upd_avars_program_eval_zbexp _ Hupd_tl).
+        * exact: (bv2z_instr_newer_than Hhd Hni_i).
+        * apply: (bv2z_upd_avars_sat_instr
+                    Hwf_i Hun_i Hni_i Hco Hsa_i Hi Hhd Hupd_hd).
+          apply: (@bvs_bvz_eqi (instr_succ_typenv i E) bs2 bs3 zs2).
+          -- apply: bvs_eqi_sym. exact: (bvs_eqi_eval_program Hun_iep Hssa_p Hp).
+          -- apply: (submap_bvz_eqi _ Heqi2).
+             exact: (ssa_unchanged_program_succ_typenv_submap Hun_iep Hssa_p).
+      + have ->: (zs_tl =
+                  (bv2z_upd_avars_program (instr_succ_typenv i E) avn g_hd' p zs_hd).2)
+          by rewrite Hupd_tl; reflexivity.
+        move: (conform_eval_succ_typenv Hwf_i Hco Hi) => Hco_3succi.
+        apply: (IH _ _ _ _ _ _ _ _ Hwf_p Hun_iep Hssa_p Hni_ie Hni_p
+                   Hco_3succi (Hsa_p bs3 Hi) Hp Htl).
+        apply: (bvz_zs_eqi Heqi2). apply: (bv2z_upd_avars_instr_eqi Hupd_hd).
+        apply: (svar_notin_replace
+                  (SSAVS.Lemmas.P.equal_sym
+                     (vars_env_program_succ_typenv p (instr_succ_typenv i E)))).
+        apply/svar_notin_union; split.
+        * apply: (svar_notin_replace
+                    (SSAVS.Lemmas.P.equal_sym (vars_env_instr_succ_typenv i E))).
+          apply/svar_notin_union. split; [exact: Hni_E | exact: Hni_lvi].
+        * exact: Hni_lvp.
+  Qed.
+
+  Lemma bv2z_upd_avars_eval_eexp {E avn g p bs e} :
+    svar_notin avn (vars_eexp e) ->
+    ZSSA.eval_zexp e (bv2z_upd_avars
+                        E avn g p (bv2z_store (program_succ_typenv p E) bs)) =
+    eval_eexp e (program_succ_typenv p E) bs.
+  Proof.
+    elim: e E g p bs => //=.
+    - move=> v E g p bs Hnotin. move: (svar_notin_singleton1 Hnotin) => Hne.
+      rewrite eq_sym in Hne. rewrite (bv2z_upd_avars_acc_ne Hne).
+      rewrite acc_bv2z_store. reflexivity.
+    - move=> op e IH E g p bs Hnotin. rewrite (IH _ _ _ _ Hnotin). reflexivity.
+    - move=> op e1 IH1 e2 IH2 E g p bs Hnotin.
+      rewrite (IH1 _ _ _ _ (svar_notin_union1 Hnotin))
+              (IH2 _ _ _ _ (svar_notin_union2 Hnotin)). reflexivity.
+  Qed.
+
+  Lemma bv2z_upd_avars_eval_ebexp {E avn g p bs e} :
+    svar_notin avn (vars_ebexp e) ->
+    ZSSA.eval_zbexp e (bv2z_upd_avars
+                         E avn g p (bv2z_store (program_succ_typenv p E) bs)) <->
+    eval_ebexp e (program_succ_typenv p E) bs.
+  Proof.
+    elim: e E g p bs => //=.
+    - move=> e1 e2 E g p bs Hnotin.
+      rewrite (bv2z_upd_avars_eval_eexp (svar_notin_union1 Hnotin))
+              (bv2z_upd_avars_eval_eexp (svar_notin_union2 Hnotin)). done.
+    - move=> e1 e2 em E g p bs Hnotin.
+      move: (svar_notin_union2 Hnotin) => Hnotin2m.
+      rewrite (bv2z_upd_avars_eval_eexp (svar_notin_union1 Hnotin))
+              (bv2z_upd_avars_eval_eexp (svar_notin_union1 Hnotin2m))
+              (bv2z_upd_avars_eval_eexp (svar_notin_union2 Hnotin2m)). done.
+    - move=> e1 IH1 e2 IH2 E g p bs Hnotin.
+      rewrite (IH1 _ _ _ _ (svar_notin_union1 Hnotin))
+              (IH2 _ _ _ _ (svar_notin_union2 Hnotin)). done.
+  Qed.
+
+
+  (* Soundness *)
+
+  Ltac decompose_svar_notin_union :=
+    repeat
+      (match goal with
+       | H : svar_notin _ (SSAVS.union _ _) |- _ =>
+         let H1 := fresh "Hni" in let H2 := fresh "Hni" in
+         move/svar_notin_union: H => [H1 H2]
+       end).
+
+  Theorem bv2z_spec_sound (o : options) (s : spec) :
+    well_formed_ssa_spec s ->
+    ssa_spec_safe s ->
+    valid_rspec (rspec_of_spec s) ->
+    ZSSA.valid_zspec (bv2z_espec o (new_svar_spec s) (espec_of_spec s)) ->
+    valid_spec s.
+  Proof.
+    destruct s as [E f p g] => /=. rewrite /well_formed_ssa_spec /bv2z_espec /=.
+    rewrite /well_formed_spec /=.
+    move/andP=> [/andP [/andP [/andP [Hwf_f Hwf_p] Hwf_g] Hunch] Hssa].
+    dcase (new_svar_spec {| sinputs := E; spre := f; sprog := p; spost := g |}) =>
+    avn Havn. set g1 := initial_index.
+    dcase (bv2z_program o E avn g1 (eqn_program p)) => [[g2 eprogs] Hzp].
+    move=> Hsafe Hrng Heqn bs1 bs2 /= Hcon [Hpre_eqn Hpre_rng] Hprog.
+
+    split; last exact: (Hrng _ _ Hcon Hpre_rng (eval_rng_program Hprog)). 
+    rewrite /ZSSA.valid_zspec /= in Heqn.
+
+    rewrite /new_svar_spec /= in Havn.
+    move: (new_svar_notin
+             (SSAVS.union (vars_env E)
+                          (SSAVS.union (vars_bexp f)
+                                       (SSAVS.union (vars_program p)
+                                                    (vars_bexp g))))).
+    rewrite Havn => Hnotin. decompose_svar_notin_union.
+    move: (svar_notin_subset (vars_ebexp_subset f) Hni1) => Hni_eqn_f.
+    move: (svar_notin_subset (vars_ebexp_subset g) Hni3) => Hni_eqn_g.
+
+    move: (SSA.well_formed_eqn_bexp Hwf_f) => Hwf_ef.
+    move/andP: Hwf_ef => [Hdef_ef Hwt_ef].
+    rewrite are_defined_subset_env in Hdef_ef.
+    move: (SSA.ssa_unchanged_program_subset Hunch Hdef_ef) => Hunch_ef.
+    rewrite -ssa_vars_unchanged_eqn_program in Hunch_ef.
+    move: (SSA.ssa_unchanged_program_eval_ebexp1
+             Hunch_ef (eval_eqn_program Hprog) Hpre_eqn) => Heval_ef.
+    move: (@bv2z_upd_avars_eval_ebexp
+             E
+             avn g1 (eqn_program p) bs2 (eqn_bexp f) Hni_eqn_f) => Hiff.
+    move: (ssa_unchanged_program_succ_typenv_submap Hunch Hssa) => Hsubmap.
+    move/andP: Hwf_f => [Hdef_f Hwt_f]. rewrite are_defined_union in Hdef_f.
+    move/andP: Hdef_f => [Hdef_eqn_f Hdef_rng_f].
+    move: (@SSA.submap_eval_ebexp _ _ _ bs2 Hsubmap Hdef_eqn_f).
+    rewrite -eqn_program_succ_typenv => H.
+    move/H/Hiff: Heval_ef => {H} Hzf.
+
+    move: (Hsafe bs1 Hpre_rng) => /= => Hsafe_at.
+    rewrite bv2z_eqn_program in Hzp.
+    move: (bv2z_upd_avars_sat_program
+             Hwf_p Hunch Hssa Hni Hni0 Hcon Hsafe_at Hprog Hzp) => Hzprog.
+    rewrite -eqn_program_succ_typenv in Hzprog.
+    rewrite -bv2z_upd_avars_eqn in Hzprog.
+
+    move: Hzf Hzprog.
+    set zbs2 := bv2z_upd_avars
+                  E avn g1 (eqn_program p)
+                  (bv2z_store (program_succ_typenv (eqn_program p) E) bs2).
+    move=> Hzf Hzprog.
+    move: (Heqn zbs2 zbs2 (conj Hzf Hzprog) (Logic.eq_refl zbs2)) => Hzg.
+
+    apply/(bv2z_upd_avars_eval_ebexp Hni_eqn_g). exact: Hzg.
+  Qed.
+
+  (* Well-formedness of bv2z_spec *)
+
+  Lemma bv2z_instr_vars_subset E o avn g1 i g2 zes :
+    well_defined_instr E i ->
+    bv2z_instr o E avn g1 i = (g2, zes) ->
+    SSAVS.subset (ZSSA.vars_zbexp (eands zes))
+                 (SSAVS.union (aux_vars_lt avn g2)
+                              (vars_env (instr_succ_typenv i E))).
+  Proof.
+    Ltac mytac ::=
+      repeat
+        match goal with
+        | H : is_true (_ && _) |- _ => hyps_splitb
+        | H : is_true (are_defined _ _) |- _ => move/defsubP: H => H
+        | |- context f [carry_constr ?o] =>
+          rewrite /carry_constr; case: (add_carry_constraints o) => /=
+        | H : bv2z_cast _ _ _ _ _ _ = _ |- _ =>
+          rewrite /bv2z_cast in H; repeat case_pairs; rewrite /=
+        | H : bv2z_vpc _ _ _ _ = _ |- _ =>
+          rewrite /bv2z_vpc in H; repeat case_pairs; rewrite /=
+        | |- context f [vars_env (SSATE.add _ _ _)] =>
+          rewrite vars_env_add_union
+        | |- context f [ZSSA.vars_zexp (bv2z_atomic _)] =>
+          rewrite vars_bv2z_atomic
+        | |- context f [ZSSA.vars_zbexp (eands (split_eand _))] =>
+          rewrite vars_eands_split_eand
+    end.
+    (case: i; rewrite /=; intros; repeat case_pairs; rewrite /=);
+      mytac; try match goal with
+                 | |- context f [aux_vars_lt ?avn (N.succ ?g)] =>
+                   let H := fresh in
+                   move/SSAVS.Lemmas.subset_singleton2:
+                     (aux_vars_lt_mem avn (N.lt_succ_diag_r g)) => H
+                 | |- context f [ZSSA.vars_zbexp (eqn_bexp ?e)] =>
+                   let H := fresh in
+                   move: (vars_ebexp_subset e) => H
+                 end;
+      by (t_auto with SSAVS.Lemmas.dp_subset).
+  Qed.
+
+  Lemma bv2z_program_vars_subset E o avn g1 p g2 eprogs :
+    well_formed_program E p ->
+    bv2z_program o E avn g1 p = (g2, eprogs) ->
+    SSAVS.subset (ZSSA.vars_zbexp (eands eprogs))
+                 (SSAVS.union (aux_vars_lt avn g2)
+                              (vars_env (program_succ_typenv p E))).
+  Proof.
+    elim: p E g1 g2 eprogs => /=.
+    - move=> ? ? ? ? _ [] _ <- /=. exact: SSAVS.Lemmas.subset_empty.
+    - move=> i p IH E g1 g2 eprogs /andP [Hwf_i Hwf_p].
+      dcase (bv2z_instr o E avn g1 i) => [[g_hd zhd] Hhd].
+      dcase (bv2z_program o (instr_succ_typenv i E) avn g_hd p) => [[g_tl ztl] Htl].
+      case=> ? ?; subst. rewrite vars_eands_cat. apply: SSAVS.Lemmas.subset_union3.
+      + rewrite vars_env_program_succ_typenv. move: (bv2z_program_idx_inc Htl) => Hg.
+        move: (aux_vars_lt_subset avn Hg) => Hsub1.
+        move/andP: Hwf_i => [Hdef_i Hwt_i].
+        move: (bv2z_instr_vars_subset Hdef_i Hhd) => Hsub2.
+        rewrite -SSAVS.Lemmas.P.union_assoc. apply: SSAVS.Lemmas.subset_union1.
+        apply: (SSAVS.Lemmas.subset_trans Hsub2). apply: SSAVS.Lemmas.subset_union3.
+        * apply: SSAVS.Lemmas.subset_union1. exact: Hsub1.
+        * apply: SSAVS.Lemmas.subset_union2. exact: SSAVS.Lemmas.subset_refl.
+      + exact: (IH _ _ _ _ Hwf_p Htl).
+  Qed.
+
+  Lemma bv2z_spec_well_formed o s :
+    well_formed_ssa_spec s ->
+    ZSSA.well_formed_zspec (bv2z_espec o (new_svar_spec s) (espec_of_spec s)).
+  Proof.
+    case: s => E f p g.
+    move=> /andP [/= /andP [/= /andP [/= /andP [Hwf_f Hwf_p] Hwf_g] Hun] Hssa].
+    rewrite /bv2z_espec /=.
+    dcase (bv2z_program
+             o E (new_svar_spec {| sinputs := E; spre := f; sprog := p; spost := g |})
+             initial_index (eqn_program p)) => [[g' eprogs] Hbvz].
+    rewrite /ZSSA.well_formed_zspec /=. rewrite andbT eqn_program_succ_typenv.
+    apply/andP; split.
+    - apply: SSAVS.Lemmas.subset_union3.
+      + apply: SSAVS.Lemmas.subset_union2.
+        move/andP: Hwf_f => [Hdef Hwt]. move/defsubP: Hdef => Hsub.
+        apply: (SSAVS.Lemmas.subset_trans (vars_ebexp_subset f)).
+        apply: (SSAVS.Lemmas.subset_trans Hsub).
+        rewrite vars_env_program_succ_typenv.
+        apply: SSAVS.Lemmas.subset_union1. exact: SSAVS.Lemmas.subset_refl.
+      + rewrite bv2z_eqn_program in Hbvz.
+        exact: (bv2z_program_vars_subset Hwf_p Hbvz).
+    - apply: SSAVS.Lemmas.subset_union1. apply: SSAVS.Lemmas.subset_union2.
+      apply: (SSAVS.Lemmas.subset_trans (vars_ebexp_subset g)).
+      move/andP: Hwf_g => [/defsubP H _]. exact: H.
+  Qed.
+
+End SplitSpec.
